WIP. fresh vars of new stratify proven correct!

coq/NNRC/Stratify/NNRCStratify.v
@@ -215,8 +215,1996 @@ Section Stratify.
    *)
 
   Section stratify.
+
+    Definition nnrc_with_substs : Type := nnrc*list (var*nnrc).
+
+    Definition mk_expr_from_vars (nws:nnrc_with_substs)
+      := fold_right (fun sdef accum => NNRCLet (fst sdef) (snd sdef) accum) (fst nws) (snd nws).
+
+    Lemma mk_expr_from_vars_eq e sdefs :
+      fold_right (fun sdef accum => NNRCLet (fst sdef) (snd sdef) accum) e sdefs = mk_expr_from_vars (e, sdefs).
+    Proof.
+      reflexivity.
+    Qed.
     
     Definition stratify1_aux
+               (body:nnrc)
+               (required_kind:nnrcKind)
+               (bound_vars:list var)
+               (sdefs:list (var*nnrc))
+      : nnrc_with_substs
+      := match required_kind with
+         | nnrcExpr =>
+           let fvar := fresh_var "stratify" bound_vars in
+           (NNRCVar fvar, sdefs++((fvar, body)::nil))
+         | _ => (body, sdefs)
+         end.
+
+    Fixpoint stratify_aux (e: nnrc) (required_kind:nnrcKind) (bound_vars:list var): nnrc_with_substs
+      := match e with
+         | NNRCGetConstant c => (e, nil)
+         | NNRCVar _ => (e, nil)
+         | NNRCConst _ => (e, nil)
+         | NNRCBinop b e1 e2 =>
+           let (e1', sdefs1) := stratify_aux e1 nnrcExpr bound_vars in
+           let bound_vars2 := (domain sdefs1) ++ bound_vars in 
+           let (e2', sdefs2) := stratify_aux e2 nnrcExpr (bound_vars2) in
+           ((NNRCBinop b e1' e2'), sdefs1++sdefs2)
+         | NNRCUnop u e1 =>
+           let (e1', sdefs1) := stratify_aux e1 nnrcExpr bound_vars in
+           ((NNRCUnop u e1'), sdefs1)
+         | NNRCLet x e1 e2 =>
+           let e1'ws := stratify_aux e1 nnrcStmt bound_vars in
+           let e1' := mk_expr_from_vars e1'ws in
+           let e2'ws := stratify_aux e2 nnrcStmt (x::bound_vars) in
+           let e2' := mk_expr_from_vars e2'ws in
+           stratify1_aux (NNRCLet x e1' e2') required_kind bound_vars nil
+         | NNRCFor x e1 e2 =>
+           let (e1', sdefs1) := stratify_aux e1 nnrcExpr bound_vars in
+           let bound_vars2 := (domain sdefs1) ++ x::bound_vars in
+           let e2'ws := stratify_aux e2 nnrcStmt (x::bound_vars) in
+           let e2' := mk_expr_from_vars e2'ws in
+           stratify1_aux (NNRCFor x e1' e2') required_kind bound_vars2 sdefs1
+         | NNRCIf e1 e2 e3 => 
+           let (e1', sdefs1) := stratify_aux e1 nnrcExpr bound_vars in
+           let bound_vars2 := (domain sdefs1) ++ bound_vars in
+           let e2'ws := stratify_aux e2 nnrcStmt bound_vars in
+           let e2' := mk_expr_from_vars e2'ws in
+           let e3'ws := stratify_aux e3 nnrcStmt bound_vars in
+           let e3' := mk_expr_from_vars e3'ws in
+           stratify1_aux (NNRCIf e1' e2' e3') required_kind bound_vars2 sdefs1
+         | NNRCEither e1 x2 e2 x3 e3 => 
+           let (e1', sdefs1) := stratify_aux e1 nnrcExpr bound_vars in
+           let bound_vars2 := (domain sdefs1) ++ bound_vars in
+           let e2'ws := stratify_aux e2 nnrcStmt (x2::bound_vars) in
+           let e2' := mk_expr_from_vars e2'ws in
+           let e3'ws := stratify_aux e3 nnrcStmt (x3::bound_vars) in
+           let e3' := mk_expr_from_vars e3'ws in
+           stratify1_aux (NNRCEither e1' x2 e2' x3 e3') required_kind (x2::x3::bound_vars2) sdefs1
+         | NNRCGroupBy s ls e1 =>
+           let (e1', sdefs1) := stratify_aux e1 nnrcExpr bound_vars in
+           stratify1_aux (NNRCGroupBy s ls e1') required_kind bound_vars sdefs1
+         end.
+
+    Definition stratify (e: nnrc) : nnrc
+      := mk_expr_from_vars (stratify_aux e nnrcStmt (nnrc_free_vars e)).
+
+  End stratify.
+  Section tests.
+    Local Open Scope nnrc_scope.
+    Local Open Scope string_scope.
+
+    Example nnrc1 := (‵abs ‵ (dnat 3) ‵+ ‵(dnat 5)) ‵+ ((‵(dnat 4) ‵+ ‵(dnat 7)) ‵+‵`(dnat  3)).
+(*    Eval vm_compute in (stratify nnrc1). *)
+
+    Example nnrc2 := NNRCLet "x" nnrc1 (NNRCVar "x").
+(*    Eval vm_compute in (stratify nnrc2). *)
+
+    Example nnrc3 := (‵abs (NNRCLet "x" ((‵(dnat 1) ‵+ ‵(dnat 2))) (((NNRCVar "x" ‵+ ‵(dnat 8)))) ‵+ ‵(dnat 5)) ‵+ ((‵(dnat 4) ‵+ ‵(dnat 7)) ‵+‵`(dnat  3))).
+(*    Eval vm_compute in (stratify nnrc3). *)
+
+    Example nnrc4 := (‵abs (NNRCFor "x" ((‵(dnat 1) ‵+ ‵(dnat 2))) (((NNRCVar "x" ‵+ ‵(dnat 8)))) ‵+ ‵(dnat 5)) ‵+ ((‵(dnat 4) ‵+ ‵(dnat 7)) ‵+‵`(dnat  3))).
+(*    Eval vm_compute in (stratify nnrc4). *)
+
+    Example nnrc5 := (‵abs (NNRCLet "z" (NNRCFor "x" ((‵(dnat 1) ‵+ ‵(dnat 2))) (((NNRCVar "x" ‵+ ‵(dnat 8)))) ‵+ ‵(dnat 5)) (NNRCVar "z")) ‵+ ((‵(dnat 4) ‵+ ‵(dnat 7)) ‵+‵`(dnat  3))).
+(*    Eval vm_compute in (stratify nnrc5). *)
+
+    Example nnrc6 := (‵abs (NNRCLet "z" (NNRCFor "x" ((‵(dnat 1) ‵+ ‵(dnat 2))) (((NNRCVar "x" ‵+ ‵(dnat 8))))) (NNRCVar "z")) ‵+ ((‵(dnat 4) ‵+ ‵(dnat 7)) ‵+‵`(dnat  3))).
+(*    Eval vm_compute in (stratify nnrc6). *)
+
+    Example nnrc7 := NNRCLet "x" (NNRCLet "y" ‵(dnat 3) (‵(dnat 8) ‵+ (NNRCVar "y"))) (NNRCVar "x").
+    
+(*    Eval vm_compute in (stratify nnrc7). *)
+
+    Example nnrc8 := NNRCLet "x" (NNRCLet "x" ‵(dnat 3) (‵(dnat 8) ‵+ (NNRCVar "x"))) (NNRCVar "x").
+    
+(*    Eval vm_compute in (stratify nnrc8). *)
+
+  End tests.
+
+  Section aux.
+    
+        Lemma incl_letvars1 v e1 e2 env :
+      incl (nnrc_vars (NNRCLet v e1 e2)) env ->
+      incl (nnrc_vars e1) env.
+    Proof.
+      intros inclvars.
+      transitivity env; unfold incl, nnrc_vars in *;
+        simpl in *; auto 2; intros.
+      apply inclvars.
+      rewrite in_app_iff in H.
+      repeat rewrite in_app_iff.
+      simpl; rewrite in_app_iff.
+      destruct H; try tauto.
+    Qed.
+    
+    Lemma incl_letvars2 v e1 e2 env :
+      incl (nnrc_vars (NNRCLet v e1 e2)) env ->
+      incl (nnrc_vars e2) (env).
+    Proof.
+      intros inclvars.
+      transitivity env; unfold incl, nnrc_vars in *;
+        simpl in *; auto 2; intros.
+      apply inclvars.
+      rewrite in_app_iff in H.
+      repeat rewrite in_app_iff.
+      simpl; rewrite in_app_iff.
+      destruct H; try tauto.
+      destruct (a == v).
+      - red in e; subst; auto.
+      - left; right.
+        apply remove_in_neq; auto.
+    Qed.
+
+        Require Import NNRCEq.
+    Require Import NNRCShadow.
+
+    Fixpoint nnrc_var_must_be_evaluated (e:nnrc) (x:var) : Prop :=
+      match e with
+      | NNRCGetConstant _ => False
+      | NNRCVar v => v = x
+      | NNRCConst _ => False
+      | NNRCBinop _ e1 e2 =>
+         nnrc_var_must_be_evaluated e1 x
+        \/ nnrc_var_must_be_evaluated e2 x
+      | NNRCUnop u e1 =>
+        nnrc_var_must_be_evaluated e1 x
+      | NNRCLet v e1 e2 =>
+        nnrc_var_must_be_evaluated e1 x
+        \/ (v <> x /\ nnrc_var_must_be_evaluated e2 x)
+      | NNRCFor v e1 e2 =>
+        nnrc_var_must_be_evaluated e1 x
+      | NNRCIf e1 e2 e3 =>
+        nnrc_var_must_be_evaluated e1 x
+      | NNRCEither e1 v2 e2 v3 e3 =>
+        nnrc_var_must_be_evaluated e1 x
+      | NNRCGroupBy g sl e1 =>
+        nnrc_var_must_be_evaluated e1 x
+      end.
+
+    Lemma nnrc_var_must_be_evaluated_dec (e:nnrc) (x:var) :
+      { nnrc_var_must_be_evaluated e x} + {~  nnrc_var_must_be_evaluated e x}.
+    Proof.
+      induction e; simpl; eauto 3.
+      - destruct (v == x); eauto.
+      - destruct IHe1; [ tauto | ].
+        destruct IHe2; [ eauto | ].
+        right; tauto.
+      - destruct IHe1; [ tauto | ].
+        destruct (x == v); unfold equiv, complement in *.
+        + right.
+          subst; intuition.
+        + destruct IHe2.
+          * left.
+            intuition.
+          * right; intuition.
+    Defined.
+
+    Lemma nnrc_must_use_preserves_failure {h:brand_relation_t} cenv e1 x e2 env :
+      disjoint (nnrc_bound_vars e2) (nnrc_free_vars e1) ->
+      nnrc_var_must_be_evaluated e2 x ->
+      @nnrc_eval _ h cenv env e1 = None ->
+      @nnrc_eval _ h cenv env (nnrc_subst e2 x e1) = None.
+    Proof.
+      revert x env.
+      induction e2; simpl; try tauto; intros x env disj me eve
+      ; unfold nnrc_eval; simpl
+        ; repeat rewrite <- nnrc_to_nnrc_base_eq.
+      - match_destr; congruence.
+      - rewrite disjoint_app_l in disj.
+        destruct disj.
+        destruct me.
+        + rewrite IHe2_1; simpl; trivial.
+        + rewrite IHe2_2; simpl; trivial.
+          apply olift2_none_r.
+      - rewrite IHe2; simpl; trivial.
+      - apply disjoint_cons_inv1 in disj.
+        rewrite disjoint_app_l in disj.
+        destruct disj as [[??]?].
+        destruct me as [me | [neq me]].
+        + rewrite IHe2_1; simpl; trivial.
+        + match_option.
+          match_destr; [congruence | ].
+          rewrite <- nnrc_to_nnrc_base_eq.
+          apply IHe2_2; trivial.
+          specialize (@nnrc_eval_remove_free_env fruntime h cenv nil v d env).
+          simpl; intros re.
+          rewrite re; trivial.
+      - apply disjoint_cons_inv1 in disj.
+        rewrite disjoint_app_l in disj.
+        destruct disj as [[??]?].
+        rewrite IHe2_1; trivial.
+      - repeat rewrite disjoint_app_l in disj.
+        destruct disj as [?[??]].
+        rewrite IHe2_1; trivial.
+      - apply disjoint_cons_inv1 in disj.
+        destruct disj as [disj ?].
+        apply disjoint_cons_inv1 in disj.
+        repeat rewrite disjoint_app_l in disj.
+        destruct disj as [[?[??]]?].
+        rewrite IHe2_1; trivial.
+      - rewrite IHe2; trivial.
+    Qed.
+        
+    Lemma let_inline_disjoint_arrow_must_use x e1 e2 :
+      disjoint (nnrc_bound_vars e2) (nnrc_free_vars e1) ->
+      nnrc_var_must_be_evaluated e2 x ->
+      nnrc_eq
+        (NNRCLet x e1 e2)
+        (nnrc_subst e2 x e1).
+    Proof.
+      red; simpl; intros.
+      unfold nnrc_eval; simpl.
+      repeat rewrite <- nnrc_to_nnrc_base_eq.
+      match_option.
+      - rewrite <- nnrc_to_nnrc_base_eq.
+        apply nnrc_eval_cons_subst_disjoint; trivial.
+      - rewrite nnrc_must_use_preserves_failure; trivial.
+    Qed.
+
+    Lemma incl_app_iff {A:Type} (l m n : list A) :
+      incl l n /\ incl m n <-> incl (l ++ m) n.
+    Proof.
+      unfold incl; intuition.
+      rewrite in_app_iff in H.
+      intuition.
+    Qed.
+
+    Lemma disjoint_with_exclusion {A:Type} (l l1 l2:list A) :
+      disjoint l1 l2 ->
+      (forall x,
+          In x l -> In x (l1 ++ l2) -> In x l1) ->
+      disjoint l l2.
+    Proof.
+      unfold disjoint; intros disj excl x inn1 inn2.
+      specialize (excl x inn1).
+      rewrite in_app_iff in excl.
+      intuition; eauto.
+    Qed.
+  
+    Lemma codomain_length  {A B:Type} (l:list (A*B)) :
+      length (codomain l) = length l.
+    Proof.
+      apply map_length.
+    Qed.
+    
+    Lemma codomain_app {A B:Type} (l₁ l₂:list (A*B)) :
+      codomain (l₁ ++ l₂) = codomain l₁ ++ codomain l₂.
+    Proof.
+      unfold codomain. rewrite map_app; trivial.
+    Qed.
+
+    Lemma app_inv_self {A:Type} (l l2:list A) :
+      l = l ++ l2 -> l2 = nil.
+    Proof.
+      intros eqq1.
+      assert (eqq2:l ++ nil = l ++ l2) by (rewrite app_nil_r; trivial).
+      apply app_inv_head in eqq2.
+      congruence.
+    Qed.
+  End aux.
+
+
+    Ltac list_simpler :=
+      repeat progress (
+      try match goal with
+      | [H: ?l  = ?l ++ _ |- _ ] => apply app_inv_self in H; try subst
+      | [H: ?l ++ _ = ?l ++ _ |- _ ] => apply app_inv_head in H; try subst
+      | [H: In _ (remove _ _ _) |- _] => apply remove_inv in H; destruct H
+      | [H: ?a <> ?v |- context [In ?a (remove _ ?v _)]] => rewrite <- (remove_in_neq _ _ _ H)
+      | [H: ?v <> ?a |- context [In ?a (remove _ ?v _)]] => rewrite <- (remove_in_neq _ a v ) by congruence
+      | [H: ?a = ?v -> False |- context [In ?a (remove _ ?v _)]] => rewrite <- (remove_in_neq _ _ _ H)
+      | [H: ?v = ?a -> False |- context [In ?a (remove _ ?v _)]] => rewrite <- (remove_in_neq _ a v) by congruence
+      end
+      ; repeat rewrite domain_app in *
+      ; repeat rewrite codomain_app in *
+      ; repeat rewrite map_app in *
+      ; repeat rewrite concat_app in *
+      ; repeat rewrite in_app_iff in *).
+      
+  Section Effective.
+
+    Lemma stratify1_aux_stratified {body required_level bv sdefs1 n sdefs2} :
+      stratify1_aux body required_level bv sdefs1 = (n,sdefs2) ->
+      stratifiedLevel nnrcStmt body ->
+      Forall (stratifiedLevel nnrcStmt) (codomain sdefs1) ->
+      stratifiedLevel required_level n /\
+      Forall (stratifiedLevel nnrcStmt) (codomain sdefs2).
+    Proof.
+      unfold stratified, stratify1_aux.
+      destruct required_level; simpl; intros eqq; invcs eqq; simpl; intuition.
+      rewrite codomain_app; simpl.
+      apply Forall_app; intuition.
+    Qed.
+
+    Lemma mk_expr_from_vars_stratified {e sdefs} :
+      stratifiedLevel nnrcStmt e ->
+      Forall (stratifiedLevel nnrcStmt) (codomain sdefs) ->
+      stratifiedLevel nnrcStmt (mk_expr_from_vars (e, sdefs)).
+    Proof.
+      unfold mk_expr_from_vars.
+      revert e; induction sdefs; intros e ste stf; simpl in *; trivial.
+      invcs stf.
+      intuition.
+    Qed.
+    
+    Lemma stratify_aux_stratified {e required_level bound_vars n sdefs} :
+      stratify_aux e required_level bound_vars = (n, sdefs) ->
+      stratifiedLevel required_level n /\
+      Forall (stratifiedLevel nnrcStmt) (codomain sdefs).
+    Proof.
+      Hint Resolve Forall_nil Forall_app.
+      revert required_level bound_vars n sdefs.
+      induction e; intros required_level bound_vars n sdefs eqq
+      ; invcs eqq; simpl in *; eauto 2; simpl.
+      - match_case_in H0;  intros ? ? eqq1; rewrite eqq1 in *.
+        match_case_in H0; intros ? ? eqq2; rewrite eqq2 in *; simpl in *.
+        invcs H0; simpl in *.
+        rewrite codomain_app.
+        destruct (IHe1 _ _ _ _ eqq1).
+        destruct (IHe2 _ _ _ _ eqq2).
+        intuition eauto.
+      - match_case_in H0;  intros ? ? eqq1; rewrite eqq1 in *; simpl in *.
+        invcs H0; simpl in *.
+        destruct (IHe _ _ _ _ eqq1).
+        intuition eauto.
+      - apply (stratify1_aux_stratified H0); simpl; eauto 2.
+        intuition.
+        + case_eq (stratify_aux e1 nnrcStmt bound_vars); intros ? ? eqq1.
+          destruct (IHe1 _ _ _ _ eqq1); simpl in *.
+          apply mk_expr_from_vars_stratified; intuition.
+        + case_eq (stratify_aux e2 nnrcStmt (v::bound_vars)); intros ? ? eqq2.
+          destruct (IHe2 _ _ _ _ eqq2); simpl in *.
+          apply mk_expr_from_vars_stratified; intuition.
+      - match_case_in H0;  intros ? ? eqq1; rewrite eqq1 in *; simpl in *.
+        destruct (IHe1 _ _ _ _ eqq1).
+        apply (stratify1_aux_stratified H0); simpl; eauto 2.
+        intuition.
+        case_eq ( (stratify_aux e2 nnrcStmt (v::bound_vars))); intros ? ? eqq2.
+        destruct (IHe2 _ _ _ _ eqq2).
+        apply mk_expr_from_vars_stratified; intuition.
+      - match_case_in H0;  intros ? ? eqq1; rewrite eqq1 in *; simpl in *.
+        destruct (IHe1 _ _ _ _ eqq1).
+        apply (stratify1_aux_stratified H0); simpl; eauto 2.
+        intuition.
+        + case_eq ( (stratify_aux e2 nnrcStmt bound_vars)); intros ? ? eqq2.
+          destruct (IHe2 _ _ _ _ eqq2).
+          apply mk_expr_from_vars_stratified; intuition.
+        + case_eq ( (stratify_aux e3 nnrcStmt bound_vars)); intros ? ? eqq3.
+          destruct (IHe3 _ _ _ _ eqq3).
+          apply mk_expr_from_vars_stratified; intuition.
+      - match_case_in H0;  intros ? ? eqq1; rewrite eqq1 in *; simpl in *.
+        destruct (IHe1 _ _ _ _ eqq1).
+        apply (stratify1_aux_stratified H0); simpl; eauto 2.
+        intuition.
+        + case_eq ( (stratify_aux e2 nnrcStmt (v::bound_vars))); intros ? ? eqq2.
+          destruct (IHe2 _ _ _ _ eqq2).
+          apply mk_expr_from_vars_stratified; intuition.
+        + case_eq ( (stratify_aux e3 nnrcStmt (v0::bound_vars))); intros ? ? eqq3.
+          destruct (IHe3 _ _ _ _ eqq3).
+          apply mk_expr_from_vars_stratified; intuition.
+      - match_case_in H0;  intros ? ? eqq1; rewrite eqq1 in *; simpl in *.
+        invcs H0; simpl in *.
+        destruct (IHe _ _ _ _ eqq1).
+        apply (stratify1_aux_stratified H1); simpl; eauto 2.
+      Qed.
+
+    Theorem stratify_stratified (e: nnrc) : stratified (stratify e).
+    Proof.
+      unfold stratify.
+      case_eq (stratify_aux e nnrcStmt nil); intros ? ? eqq1.
+      destruct (stratify_aux_stratified eqq1).
+      apply mk_expr_from_vars_stratified; simpl; eauto.
+    Qed.
+
+    Corollary stratify_stratified_spec (e: nnrc) : stratified_spec (stratify e).
+    Proof.
+      apply stratified_correct.
+      apply stratify_stratified.
+    Qed.
+
+  End Effective.
+
+  Section Idempotent.
+
+    Lemma mk_expr_from_vars_nil e : 
+      mk_expr_from_vars (e, nil) = e.
+    Proof.
+      reflexivity.
+    Qed.
+    
+    Lemma stratify_aux_stratify_id
+          (e: nnrc)
+          (required_level:nnrcKind)
+          (bound_vars:list var) :
+      stratifiedLevel required_level e -> 
+      stratify_aux e required_level bound_vars = (e, nil).
+    Proof.
+      revert required_level bound_vars.
+      induction e; intros required_level bound_vars stratify_levelc; simpl in *; trivial.
+      - rewrite IHe1, IHe2 by tauto.
+        simpl; trivial.
+      - rewrite IHe by tauto.
+        simpl; trivial.
+      - rewrite IHe1, IHe2 by tauto; simpl.
+        repeat rewrite mk_expr_from_vars_nil.
+        intuition; subst; simpl; trivial.
+      - rewrite IHe1, IHe2 by tauto; simpl.
+        repeat rewrite mk_expr_from_vars_nil.
+        intuition; subst; simpl; trivial.
+      - rewrite IHe1, IHe2, IHe3 by tauto; simpl.
+        repeat rewrite mk_expr_from_vars_nil.
+        intuition; subst; simpl; trivial.
+      - rewrite IHe1, IHe2, IHe3 by tauto; simpl.
+        repeat rewrite mk_expr_from_vars_nil.
+        intuition; subst; simpl; trivial.
+      - rewrite IHe by tauto.
+        intuition; subst; simpl; trivial.
+    Qed.
+
+    Theorem stratify_stratify_id (e: nnrc) :
+      stratified e ->              
+      stratify e = e.
+    Proof.
+      unfold stratify.
+      intros stratifye.
+      rewrite (stratify_aux_stratify_id _ _ _ stratifye).
+      rewrite mk_expr_from_vars_nil.
+      trivial.
+    Qed.
+
+    Corollary stratify_idem (e: nnrc) :
+      stratify (stratify e) = stratify e.
+    Proof.
+      apply stratify_stratify_id.
+      apply stratify_stratified.
+    Qed.
+
+  End Idempotent.
+
+  Section BoundVars.
+
+        Lemma stratify1_aux_nbound_vars {e required_kind bound_vars n l sdefs} :
+      stratify1_aux e required_kind bound_vars sdefs = (n,l) ->
+      forall x, In x (domain l) -> In x bound_vars -> In x (domain sdefs).
+    Proof.
+      destruct required_kind; simpl; trivial; intros eqq ? inn; invcs eqq; trivial.
+      intros.
+      rewrite domain_app, in_app_iff in inn.
+      destruct inn; trivial.
+      - simpl in *.
+        destruct H0; try tauto.
+        subst.
+        apply fresh_var_fresh in H.
+        tauto.
+    Qed.
+
+    Lemma stratify_aux_nbound_vars {e required_kind bound_vars n sdefs} :
+      stratify_aux e required_kind bound_vars = (n,sdefs) ->
+      disjoint (domain sdefs) bound_vars.
+    Proof.
+      revert required_kind bound_vars sdefs n; induction e; intros required_kind bound_vars sdefs n eqq; simpl in eqq; invcs eqq; simpl
+      ; try apply disjoint_nil_l.
+      - match_case_in H0; intros ? ? eqq1
+        ; rewrite eqq1 in H0.
+         match_case_in H0; intros ? ? eqq2
+         ; rewrite eqq2 in H0.
+         invcs H0.
+         rewrite domain_app, disjoint_app_l.
+         split; eauto.
+         specialize (IHe2 _ _ _ _ eqq2).
+         rewrite disjoint_app_r in IHe2.
+         intuition.
+      -  match_case_in H0; intros ? ? eqq1
+         ; rewrite eqq1 in H0.
+         invcs H0.
+         eauto.
+      - specialize (stratify1_aux_nbound_vars H0); intros HH.
+        eauto.
+      - match_case_in H0; intros ? ? eqq1
+        ; rewrite eqq1 in H0.
+        specialize (IHe1 _ _ _ _ eqq1).
+        specialize (stratify1_aux_nbound_vars H0); intros HH.
+        eapply disjoint_with_exclusion; eauto.
+        intuition; list_simpler; intuition.
+      - match_case_in H0; intros ? ? eqq1
+        ; rewrite eqq1 in H0.
+        specialize (IHe1 _ _ _ _ eqq1).
+        specialize (stratify1_aux_nbound_vars H0); intros HH.
+        eapply disjoint_with_exclusion; eauto.
+      - match_case_in H0; intros ? ? eqq1
+        ; rewrite eqq1 in H0.
+        specialize (IHe1 _ _ _ _ eqq1).
+        specialize (stratify1_aux_nbound_vars H0); intros HH.
+        eapply disjoint_with_exclusion; eauto.
+        intuition; list_simpler; intuition.
+      - match_case_in H0; intros ? ? eqq1
+         ; rewrite eqq1 in H0.
+        invcs H0.
+        specialize (stratify1_aux_nbound_vars H1); intros HH.
+        eapply disjoint_with_exclusion; eauto.
+        intuition; list_simpler; intuition.
+    Qed.
+
+  End BoundVars.
+
+  Section FreeVars.
+
+    Fixpoint growing_fv_ctxt (l:list (var*nnrc)) (ctxt:list var) : Prop
+      := match l with
+         | nil => True
+         | (v,e)::lx =>
+           incl (nnrc_free_vars e) ctxt
+           /\ growing_fv_ctxt lx (v::ctxt)
+         end.
+
+    Require Import Program.Basics.
+    
+    Global Instance growing_fv_ctxt_incl :
+      Proper (eq ==> (@incl var) ==> impl) growing_fv_ctxt.
+    Proof.
+      unfold Proper, respectful, flip, impl. intros ? sdefs ? ctxt1 ctxt2; subst.
+      revert ctxt1 ctxt2.
+      induction sdefs; simpl; trivial; intros.
+      destruct a; simpl.
+      intuition.
+      - rewrite H1; trivial.
+      - eapply IHsdefs; eauto.
+        red; simpl; intuition.
+    Qed.
+
+    Global Instance growing_fv_ctxt_equiv :
+      Proper (eq ==> (@equivlist var) ==> iff) growing_fv_ctxt.
+    Proof.
+      unfold Proper, respectful, flip, impl. intros ? sdefs ? ctxt1 ctxt2; subst; intros eqq.
+      apply equivlist_incls in eqq.
+      destruct eqq.
+      split; intro HH; eapply growing_fv_ctxt_incl; eauto.
+    Qed.
+
+    Lemma growing_fv_ctxt_app sdefs1 sdefs2 ctxt :
+          growing_fv_ctxt (sdefs1 ++ sdefs2) ctxt <->
+          (growing_fv_ctxt sdefs1 ctxt /\ growing_fv_ctxt sdefs2 (ctxt ++ domain sdefs1)).
+    Proof.
+      revert ctxt sdefs2; induction sdefs1; intros ctxt sdefs2; simpl.
+      - rewrite app_nil_r. intuition.
+      - destruct a; simpl.
+        rewrite IHsdefs1; simpl.
+        assert (eqv: equivlist (v :: ctxt ++ domain sdefs1) (ctxt ++ v :: domain sdefs1))
+          by (intro; simpl; repeat rewrite in_app_iff; simpl; intuition).
+        rewrite eqv.
+        intuition.
+    Qed.
+
+        Lemma mk_expr_from_vars_growing_fv_free_fw {sdefs ctxt} :
+      growing_fv_ctxt sdefs ctxt ->
+      forall e x,
+        In x (nnrc_free_vars (mk_expr_from_vars (e, sdefs))) ->
+        ((In x (nnrc_free_vars e) /\ ~ In x (domain sdefs)) \/ In x ctxt).
+    Proof.
+      revert ctxt ; induction sdefs; intros ctxt gfc e x inn; [intuition | ].
+      destruct a.
+      simpl in *; rewrite mk_expr_from_vars_eq in inn.
+      destruct gfc as [incln gfc].
+      rewrite in_app_iff in inn.
+      destruct inn as [inn|inn]; [intuition | ].
+      apply remove_inv in inn.
+      destruct inn as [inn neq].
+      specialize (IHsdefs _ gfc _ _ inn).
+      destruct IHsdefs as [[inn2 inn3] | inn2]; simpl in *; intuition. 
+    Qed.
+
+    Lemma mk_expr_from_vars_growing_fv_free_fw_codomain {sdefs e x} :
+        In x (nnrc_free_vars (mk_expr_from_vars (e, sdefs))) ->
+        ((In x (nnrc_free_vars e) \/ In x (concat (map nnrc_free_vars (codomain sdefs))))).
+    Proof.
+      revert e x ; induction sdefs; intros e x inn; [intuition | ].
+      destruct a.
+      simpl in *; rewrite mk_expr_from_vars_eq in inn.
+      list_simpler.
+      intuition.
+      list_simpler.
+      apply IHsdefs in H.
+      intuition.
+    Qed.
+
+    Lemma mk_expr_from_vars_growing_fv_free_bk e sdefs x :
+        ((In x (nnrc_free_vars e) \/ In x (concat (map nnrc_free_vars (codomain sdefs)))) /\ ~ In x (domain sdefs)) ->
+        In x (nnrc_free_vars (mk_expr_from_vars (e, sdefs))).
+    Proof.
+      unfold mk_expr_from_vars.
+      revert e x; induction sdefs; intros e x inn; [intuition | ].
+      destruct a.
+      simpl in *; rewrite mk_expr_from_vars_eq in *.
+      list_simpler.
+      specialize (IHsdefs e x); intuition.
+      rewrite mk_expr_from_vars_eq in *.
+      list_simpler.
+      intuition.
+      rewrite mk_expr_from_vars_eq in *.
+      list_simpler.
+      intuition.
+    Qed.
+
+    Lemma stratify1_aux_free_vars_incl {e required_level bound_vars n sdefs1 sdefs2} :
+      stratify1_aux e required_level bound_vars sdefs1 = (n, sdefs2) ->
+      incl (nnrc_free_vars n) (nnrc_free_vars e ++ (domain sdefs2)).
+    Proof.
+      destruct required_level; simpl; intros eqq; invcs eqq; simpl.
+      - intros ? inn; simpl in inn; intuition.
+        subst.
+        rewrite domain_app.
+        repeat rewrite in_app_iff; simpl; intuition.
+      - apply incl_appl; reflexivity.
+    Qed.
+
+    Lemma stratify1_aux_sdefs_app {e required_level bound_vars n sdefs1 sdefs2} :
+      stratify1_aux e required_level bound_vars sdefs1 = (n, sdefs2) ->
+      { l | sdefs2 = sdefs1++l}.
+    Proof.
+      destruct required_level; simpl; intros eqq; invcs eqq; simpl.
+      - eauto.
+      - exists nil.
+        rewrite app_nil_r; trivial.
+    Defined.
+
+    Lemma stratify1_aux_gfc {e required_level bound_vars n sdefs1 sdefs2} :
+      stratify1_aux e required_level bound_vars sdefs1 = (n, sdefs2) ->
+      forall ctxt,
+      growing_fv_ctxt sdefs1 ctxt ->
+      growing_fv_ctxt sdefs2 (ctxt++nnrc_free_vars e).
+    Proof.
+      destruct required_level; simpl; intros HH gfc; invcs HH.
+      - rewrite growing_fv_ctxt_app; simpl.
+        intuition.
+        eapply growing_fv_ctxt_incl; eauto
+        ; intros ?; repeat rewrite in_app_iff; intuition.
+      - eapply growing_fv_ctxt_incl; eauto
+        ; intros ?; repeat rewrite in_app_iff; intuition.
+    Qed.
+
+    Lemma stratify1_aux_gfc_weak {e required_level bound_vars n sdefs1 sdefs2} :
+      stratify1_aux e required_level bound_vars sdefs1 = (n, sdefs2) ->
+      growing_fv_ctxt sdefs1 (nnrc_free_vars e) ->
+      growing_fv_ctxt sdefs2 (nnrc_free_vars e).
+    Proof.
+      intros gfc eqq.
+      generalize (stratify1_aux_gfc gfc _ eqq); intros HH.
+      - eapply growing_fv_ctxt_incl; eauto
+        ; intros ?; repeat rewrite in_app_iff; intuition.
+    Qed.
+
+    Lemma stratify1_aux_gfc_app {e required_level bound_vars n sdefs1 sdefs2} :
+      stratify1_aux e required_level bound_vars sdefs1 = (n, sdefs1++sdefs2) ->
+      forall ctxt,
+      growing_fv_ctxt sdefs1 ctxt ->
+      growing_fv_ctxt sdefs2 (ctxt++nnrc_free_vars e).
+    Proof.
+      destruct required_level; simpl; intros HH gfc; invcs HH.
+      - apply app_inv_head in H1.
+        invcs H1; simpl.
+        split; trivial.
+        intros ?; repeat rewrite in_app_iff; intuition.
+      - assert (mknil:sdefs1++nil = sdefs1++sdefs2) by (rewrite app_nil_r; trivial).
+        apply app_inv_head in mknil; subst.
+        simpl; trivial.
+    Qed.
+
+    Lemma stratify1_aux_gfc_app_weak {e required_level bound_vars n sdefs1 sdefs2} :
+      stratify1_aux e required_level bound_vars sdefs1 = (n, sdefs1++sdefs2) ->
+      growing_fv_ctxt sdefs1 (nnrc_free_vars e) ->
+      growing_fv_ctxt sdefs2 (nnrc_free_vars e).
+    Proof.
+      intros eqq gfc.
+      generalize (stratify1_aux_gfc_app eqq _ gfc); intros HH.
+      - eapply growing_fv_ctxt_incl; eauto
+        ; intros ?; repeat rewrite in_app_iff; intuition.
+    Qed.
+
+    Lemma mk_expr_from_vars_has_codomain_vars a l n :
+      In a (concat (map nnrc_free_vars (codomain l))) ->
+         ~ In a (domain l) ->
+         In a (nnrc_free_vars (mk_expr_from_vars (n, l))).
+    Proof.
+      unfold mk_expr_from_vars.
+      revert a n.
+      induction l; simpl; intuition.
+      simpl in *.
+      list_simpler.
+      intuition.
+    Qed.
+
+    Lemma stratify1_aux_free_vars {e required_level bound_vars n}
+                                     {sdefs1 sdefs2:list (var*nnrc)} :
+      stratify1_aux e required_level bound_vars sdefs1 = (n, sdefs1++sdefs2) ->
+      equivlist (nnrc_free_vars n ++ (concat (map nnrc_free_vars (codomain sdefs2)))) (nnrc_free_vars e ++ (domain sdefs2)).
+    Proof.
+      destruct required_level; simpl; intros eqq; invcs eqq; simpl
+      ; list_simpler; simpl in *.
+      - red; split; simpl; list_simpler; simpl; eauto; intuition.
+      - reflexivity.
+    Qed.
+
+    Lemma stratify_aux_free_vars_and_growing
+          {e required_level bound_vars n sdefs} :
+      stratify_aux e required_level bound_vars = (n,sdefs) ->
+      incl (nnrc_free_vars e) bound_vars ->
+      equivlist (nnrc_free_vars n ++ (concat (map nnrc_free_vars (codomain sdefs)))) (nnrc_free_vars e ++ domain sdefs)
+      /\ growing_fv_ctxt sdefs (nnrc_free_vars e).
+    Proof.
+      unfold equivlist.
+      revert required_level bound_vars sdefs n.
+      induction e; intros required_level bound_vars sdefs n eqq inclb
+      ; simpl in *; invcs eqq; simpl; unfold incl; try tauto.
+      - match_case_in H0; intros ? ? eqq1; rewrite eqq1 in H0.
+        match_case_in H0; intros ? ? eqq2; rewrite eqq2 in H0.
+        invcs H0; simpl.
+        apply incl_app_iff in inclb.
+        destruct inclb as [inclb1 inclb2].
+        destruct (IHe1 _ _ _ _ eqq1 inclb1) as [IHe1i IHe1g].
+        assert (inclb2':incl (nnrc_free_vars e2) (domain l ++ bound_vars))
+               by (intros ? inn; list_simpler; intuition).
+        specialize (IHe2 _ _ _ _ eqq2 inclb2') as [IHe2i IHe2g].
+        list_simpler.
+        split. 
+        + intros a. specialize (IHe1i a). specialize (IHe2i a).
+          repeat rewrite in_app_iff in *.
+          intuition.
+        + rewrite growing_fv_ctxt_app; split.
+          * eapply growing_fv_ctxt_incl; eauto
+            ; intros ?; repeat rewrite in_app_iff; intuition.
+          * eapply growing_fv_ctxt_incl; eauto
+            ; intros ?; repeat rewrite in_app_iff; intuition.
+      - match_case_in H0; intros ? ? eqq1; rewrite eqq1 in H0.
+        invcs H0; simpl.
+        destruct (IHe _ _ _ _ eqq1 inclb) as [IHe1i IHe1g].
+        intuition.
+      - destruct (stratify1_aux_sdefs_app H0) as [sdefs' ?]; subst.
+        generalize (stratify1_aux_free_vars H0); simpl; intros HH.
+        case_eq (stratify_aux e1 nnrcStmt bound_vars); intros ? ? eqq1.
+        case_eq (stratify_aux e2 nnrcStmt (v::bound_vars)); intros ? ? eqq2.
+        rewrite eqq1 in *; rewrite eqq2 in *.
+        destruct (IHe1 _ _ _ _ eqq1) as [IHe1i IHe1g].
+        { intros a; specialize (inclb a); list_simpler; intuition. }
+        destruct (IHe2 _ _ _ _ eqq2) as [IHe2i IHe2g].
+        { intros a; specialize (inclb a); simpl; list_simpler.
+          destruct (v == a); unfold equiv, complement in *.
+          - subst; eauto.
+          - intros inn; right; apply inclb.
+            list_simpler; tauto.
+        }
+        split. 
+        + intros a; rewrite (HH a); clear HH.
+          specialize (IHe1i a); specialize (IHe2i a).
+          list_simpler.
+          split; intros inn.
+          * { intuition.
+              - generalize (mk_expr_from_vars_growing_fv_free_fw IHe1g _ _ H5)
+                ; intros HH.
+                intuition.
+              - list_simpler.
+                generalize (mk_expr_from_vars_growing_fv_free_fw IHe2g _ _ H3)
+                ; intros HH.
+                intuition.
+            }
+          * { destruct inn as [inn|inn]; try tauto.
+              destruct inn as [inn|inn].
+              - assert (adisj:~ In a (domain l)).
+                { generalize (stratify_aux_nbound_vars eqq1); intros disj.
+                  specialize (disj a).
+                  intros innd; apply (disj innd).
+                  apply inclb; list_simpler; tauto.
+                } 
+                generalize (mk_expr_from_vars_growing_fv_free_bk n0 l a); intros HH.
+                destruct IHe1i as [IHe1if IHe1ib].
+                cut_to IHe1ib; try tauto.
+              - list_simpler.
+                assert (adisj:~ In a (domain l0)).
+                { generalize (stratify_aux_nbound_vars eqq2); intros disj.
+                  specialize (disj a).
+                  intros innd; apply (disj innd).
+                  simpl; right.
+                  apply inclb; list_simpler; tauto.
+                } 
+                generalize (mk_expr_from_vars_growing_fv_free_bk n1 l0 a); intros HH.
+                destruct IHe2i as [IHe2if IHe2ib].
+                cut_to IHe2ib; try tauto.
+            }
+        + generalize (stratify1_aux_gfc_app_weak H0); simpl; intros HH2.
+          specialize (HH2 I).
+          * { eapply growing_fv_ctxt_incl; eauto
+              ; intros ?; repeat rewrite in_app_iff; intuition.
+              -
+                generalize (mk_expr_from_vars_growing_fv_free_fw IHe1g _ _ H1)
+                ; intros HH3.
+                specialize (IHe1i a).
+                list_simpler.
+                intuition.
+              - list_simpler.
+                generalize (mk_expr_from_vars_growing_fv_free_fw IHe2g _ _ H)
+                ; intros HH3.
+                specialize (IHe2i a).
+                list_simpler.
+                intuition.
+            }
+      - match_case_in H0; intros ? ? eqq1; rewrite eqq1 in H0.
+        destruct (stratify1_aux_sdefs_app H0) as [sdefs' ?]; subst.
+        generalize (stratify1_aux_free_vars H0); simpl; intros HH.
+        case_eq (stratify_aux e2 nnrcStmt (v::bound_vars)); intros ? ? eqq2.
+        rewrite eqq2 in *.
+        destruct (IHe1 _ _ _ _ eqq1) as [IHe1i IHe1g].
+        { intros a; specialize (inclb a); list_simpler; intuition. }
+        destruct (IHe2 _ _ _ _ eqq2) as [IHe2i IHe2g].
+        { intros a; specialize (inclb a); simpl; list_simpler.
+          destruct (v == a); unfold equiv, complement in *.
+          - subst; eauto.
+          - intros inn; right; apply inclb.
+            list_simpler; tauto.
+        }
+        split. 
+        + intros a; specialize (HH a).
+          specialize (IHe1i a); specialize (IHe2i a).
+          list_simpler.
+          split; intros inn.
+          * { destruct inn as [inn|[inn|inn]].
+              - destruct HH as [HHf _].
+                cut_to HHf; [ | tauto].
+                destruct HHf; [ | tauto].
+                destruct H; [tauto | ].
+                list_simpler.
+                generalize (mk_expr_from_vars_growing_fv_free_fw IHe2g _ _ H)
+                ; intros HH.
+                intuition.
+              - revert IHe1i inn; clear; intuition.
+              - destruct HH as [HHf _].
+                cut_to HHf; [ | tauto].
+                destruct HHf; [ | tauto].
+                destruct H; [tauto | ].
+                list_simpler.
+                generalize (mk_expr_from_vars_growing_fv_free_fw IHe2g _ _ H)
+                ; intros HH.
+                intuition.
+            } 
+          * { destruct inn as [inn|inn]; [ | tauto ].
+              destruct inn as [inn|inn]; [ tauto | ].
+              - list_simpler.
+                assert (adisj:~ In a (domain l0)).
+                { generalize (stratify_aux_nbound_vars eqq2); intros disj.
+                  specialize (disj a).
+                  intros innd; apply (disj innd).
+                  simpl; right.
+                  apply inclb; list_simpler; tauto.
+                } 
+                destruct IHe2i as [IHe2if IHe2ib].
+                cut_to IHe2ib; try tauto.
+                generalize (mk_expr_from_vars_growing_fv_free_bk n1 l0 a); intros HH2.
+                cut_to HH2; [ | tauto].
+                destruct HH as [HHf HHb].
+                cut_to HHb; [ | list_simpler; tauto].
+                tauto.
+            }
+        + rewrite growing_fv_ctxt_app; split.
+          * eapply growing_fv_ctxt_incl; eauto
+            ; intros ?; repeat rewrite in_app_iff; intuition.
+          * generalize (stratify1_aux_gfc_app H0 _ IHe1g); intros HH2.
+            simpl in HH2.
+            eapply growing_fv_ctxt_incl; eauto
+            ; intros ?; repeat rewrite in_app_iff.
+            intros inn.
+            destruct inn as [?|inn]; [tauto | ].
+            { destruct inn.
+              - specialize (IHe1i a); list_simpler; tauto.
+              - list_simpler.
+                generalize (mk_expr_from_vars_growing_fv_free_fw IHe2g _ _ H)
+                ; intros HH3.
+                specialize (IHe2i a).
+                list_simpler.
+                intuition.
+            }
+      - match_case_in H0; intros ? ? eqq1; rewrite eqq1 in H0.
+        destruct (stratify1_aux_sdefs_app H0) as [sdefs' ?]; subst.
+        generalize (stratify1_aux_free_vars H0); simpl; intros HH.
+        case_eq (stratify_aux e2 nnrcStmt bound_vars); intros ? ? eqq2.
+        rewrite eqq2 in *.
+        case_eq (stratify_aux e3 nnrcStmt bound_vars); intros ? ? eqq3.
+        rewrite eqq3 in *.
+        destruct (IHe1 _ _ _ _ eqq1) as [IHe1i IHe1g].
+        { intros a; specialize (inclb a); list_simpler; intuition. }
+        destruct (IHe2 _ _ _ _ eqq2) as [IHe2i IHe2g].
+        { intros a; specialize (inclb a); simpl; list_simpler; intuition. }
+        destruct (IHe3 _ _ _ _ eqq3) as [IHe3i IHe3g].
+        { intros a; specialize (inclb a); simpl; list_simpler; intuition. }
+        split. 
+        + intros a; specialize (HH a).
+          specialize (IHe1i a); specialize (IHe2i a); specialize (IHe3i a).
+          list_simpler.
+          split; intros inn.
+          * { destruct inn as [inn|[inn|inn]].
+              - destruct HH as [HHf _].
+                cut_to HHf; [ | tauto].
+                destruct HHf; [ | tauto].
+                destruct H; [tauto | ].
+                list_simpler.
+                destruct H.
+                + generalize (mk_expr_from_vars_growing_fv_free_fw IHe2g _ _ H)
+                  ; intuition.
+                + generalize (mk_expr_from_vars_growing_fv_free_fw IHe3g _ _ H)
+                  ; intuition.
+              - revert IHe1i inn; clear; intuition.
+              - destruct HH as [HHf _].
+                cut_to HHf; [ | tauto].
+                destruct HHf; [ | tauto].
+                destruct H; [tauto | ].
+                list_simpler.
+                destruct H.
+                + generalize (mk_expr_from_vars_growing_fv_free_fw IHe2g _ _ H)
+                  ; intuition.
+                + generalize (mk_expr_from_vars_growing_fv_free_fw IHe3g _ _ H)
+                  ; intuition.
+            } 
+          * { destruct inn as [inn|inn]; [ | tauto ].
+              destruct inn as [inn|inn]; [ tauto | ].
+              - list_simpler.
+                destruct inn as [inn|inn].
+                + assert (adisj:~ In a (domain l0)).
+                  { generalize (stratify_aux_nbound_vars eqq2); intros disj.
+                    specialize (disj a).
+                    intros innd; apply (disj innd).
+                    apply inclb; list_simpler.
+                    revert inn; clear; tauto.
+                  }
+                destruct IHe2i as [IHe2if IHe2ib].
+                cut_to IHe2ib; try tauto.
+                generalize (mk_expr_from_vars_growing_fv_free_bk n1 l0 a); intros HH2.
+                cut_to HH2; [ | revert IHe2ib adisj; clear; tauto].
+                destruct HH as [HHf HHb].
+                cut_to HHb; [ | list_simpler].
+                * revert HHb; clear; tauto.
+                * revert HH2; clear; tauto.
+                + assert (adisj:~ In a (domain l1)).
+                  { generalize (stratify_aux_nbound_vars eqq3); intros disj.
+                    specialize (disj a).
+                    intros innd; apply (disj innd).
+                    apply inclb; list_simpler.
+                    revert inn; clear; tauto.
+                  }
+                destruct IHe3i as [IHe3if IHe3ib].
+                cut_to IHe3ib; try tauto.
+                generalize (mk_expr_from_vars_growing_fv_free_bk n2 l1 a); intros HH3.
+                cut_to HH3; [ | revert IHe3ib adisj; clear; tauto].
+                destruct HH as [HHf HHb].
+                cut_to HHb; [ | list_simpler].
+                * revert HHb; clear; tauto.
+                * revert HH3; clear; tauto.
+            }
+        + rewrite growing_fv_ctxt_app; split.
+          * eapply growing_fv_ctxt_incl; eauto
+            ; intros ?; repeat rewrite in_app_iff; intuition.
+          * generalize (stratify1_aux_gfc_app H0 _ IHe1g); intros HH2.
+            simpl in HH2.
+            eapply growing_fv_ctxt_incl; eauto
+            ; intros ?; repeat rewrite in_app_iff.
+            intros inn.
+            destruct inn as [?|inn]; [tauto | ].
+            { destruct inn as [inn|[inn|inn]].
+              - specialize (IHe1i a); list_simpler; tauto.
+              - list_simpler.
+                generalize (mk_expr_from_vars_growing_fv_free_fw IHe2g _ _ inn)
+                ; intros HH3.
+                specialize (IHe2i a).
+                list_simpler.
+                intuition.
+              - list_simpler.
+                generalize (mk_expr_from_vars_growing_fv_free_fw IHe3g _ _ inn)
+                ; intros HH3.
+                specialize (IHe3i a).
+                list_simpler.
+                intuition.
+            }
+      - match_case_in H0; intros ? ? eqq1; rewrite eqq1 in H0.
+        destruct (stratify1_aux_sdefs_app H0) as [sdefs' ?]; subst.
+        generalize (stratify1_aux_free_vars H0); simpl; intros HH.
+        case_eq (stratify_aux e2 nnrcStmt (v::bound_vars)); intros ? ? eqq2.
+        rewrite eqq2 in *.
+        case_eq (stratify_aux e3 nnrcStmt (v0::bound_vars)); intros ? ? eqq3.
+        rewrite eqq3 in *.
+        destruct (IHe1 _ _ _ _ eqq1) as [IHe1i IHe1g].
+        { intros a; specialize (inclb a); list_simpler; intuition. }
+        destruct (IHe2 _ _ _ _ eqq2) as [IHe2i IHe2g].
+        { intros a; specialize (inclb a); simpl; list_simpler.
+          destruct (v == a); unfold equiv, complement in *.
+          - subst; eauto.
+          - intros inn; right; apply inclb.
+            list_simpler; tauto.
+        }
+        destruct (IHe3 _ _ _ _ eqq3) as [IHe3i IHe3g].
+        { intros a; specialize (inclb a); simpl; list_simpler.
+          destruct (v0 == a); unfold equiv, complement in *.
+          - subst; eauto.
+          - intros inn; right; apply inclb.
+            list_simpler; tauto.
+        }
+        split. 
+        + intros a; specialize (HH a).
+          specialize (IHe1i a); specialize (IHe2i a); specialize (IHe3i a).
+          list_simpler.
+          split; intros inn.
+          * { destruct inn as [inn|[inn|inn]].
+              - destruct HH as [HHf _].
+                cut_to HHf; [ | tauto].
+                destruct HHf; [ | tauto].
+                destruct H; [tauto | ].
+                destruct H; list_simpler.
+                + generalize (mk_expr_from_vars_growing_fv_free_fw IHe2g _ _ H)
+                  ; intuition.
+                + generalize (mk_expr_from_vars_growing_fv_free_fw IHe3g _ _ H)
+                  ; intuition.
+              - revert IHe1i inn; clear; intuition.
+              - destruct HH as [HHf _].
+                cut_to HHf; [ | tauto].
+                destruct HHf; [ | tauto].
+                destruct H; [tauto | ].
+                destruct H; list_simpler.
+                + generalize (mk_expr_from_vars_growing_fv_free_fw IHe2g _ _ H)
+                  ; intuition.
+                + generalize (mk_expr_from_vars_growing_fv_free_fw IHe3g _ _ H)
+                  ; intuition.
+            } 
+          * { destruct inn as [inn|inn]; [ | tauto ].
+              destruct inn as [inn|inn]; [ tauto | ].
+              - list_simpler.
+                destruct inn as [inn|inn].
+                + assert (adisj:~ In a (domain l0)).
+                  { generalize (stratify_aux_nbound_vars eqq2); intros disj.
+                    specialize (disj a).
+                    intros innd; apply (disj innd).
+                    simpl; right.
+                    apply inclb; list_simpler.
+                    revert H; clear; tauto.
+                  }
+                destruct IHe2i as [IHe2if IHe2ib].
+                cut_to IHe2ib; try tauto.
+                generalize (mk_expr_from_vars_growing_fv_free_bk n1 l0 a); intros HH2.
+                cut_to HH2; [ | revert IHe2ib adisj; clear; tauto].
+                destruct HH as [HHf HHb].
+                cut_to HHb; [ | list_simpler].
+                * revert HHb; clear; tauto.
+                * revert HH2; clear; tauto.
+                * list_simpler; revert H; clear; tauto.
+                + assert (adisj:~ In a (domain l1)).
+                  { generalize (stratify_aux_nbound_vars eqq3); intros disj.
+                    specialize (disj a).
+                    intros innd; apply (disj innd).
+                    simpl; right.
+                    apply inclb; list_simpler.
+                    revert H; clear; tauto.
+                  }
+                destruct IHe3i as [IHe3if IHe3ib].
+                cut_to IHe3ib; try tauto.
+                generalize (mk_expr_from_vars_growing_fv_free_bk n2 l1 a); intros HH3.
+                cut_to HH3; [ | revert IHe3ib adisj; clear; tauto].
+                destruct HH as [HHf HHb].
+                cut_to HHb; [ | list_simpler].
+                * revert HHb; clear; tauto.
+                * revert HH3; clear; tauto.
+                * list_simpler; revert H; clear; tauto.
+            }
+        + rewrite growing_fv_ctxt_app; split.
+          * eapply growing_fv_ctxt_incl; eauto
+            ; intros ?; repeat rewrite in_app_iff; intuition.
+          * generalize (stratify1_aux_gfc_app H0 _ IHe1g); intros HH2.
+            simpl in HH2.
+            eapply growing_fv_ctxt_incl; eauto
+            ; intros ?; repeat rewrite in_app_iff.
+            intros inn.
+            destruct inn as [?|inn]; [tauto | ].
+            { destruct inn as [inn|[inn|inn]].
+              - specialize (IHe1i a); list_simpler; tauto.
+              - list_simpler.
+                generalize (mk_expr_from_vars_growing_fv_free_fw IHe2g _ _ H)
+                ; intros HH3.
+                specialize (IHe2i a).
+                list_simpler.
+                intuition.
+              - list_simpler.
+                generalize (mk_expr_from_vars_growing_fv_free_fw IHe3g _ _ H)
+                ; intros HH3.
+                specialize (IHe3i a).
+                list_simpler.
+                intuition.
+            }
+      - match_case_in H0; intros ? ? eqq1; rewrite eqq1 in H0.
+        destruct (stratify1_aux_sdefs_app H0) as [sdefs' ?]; subst.
+        generalize (stratify1_aux_free_vars H0); simpl; intros HH.
+        destruct (IHe _ _ _ _ eqq1) as [IHe1i IHe1g].
+        { intros a; specialize (inclb a); list_simpler; intuition. }
+        split. 
+        + intros a; specialize (HH a).
+          specialize (IHe1i a).
+          list_simpler.
+          tauto.
+        + rewrite growing_fv_ctxt_app; split.
+          * eapply growing_fv_ctxt_incl; eauto
+            ; intros ?; repeat rewrite in_app_iff; intuition.
+          * generalize (stratify1_aux_gfc_app H0 _ IHe1g); intros HH2.
+            simpl in HH2.
+            eapply growing_fv_ctxt_incl; eauto
+            ; intros ?; repeat rewrite in_app_iff.
+            intros inn.
+            destruct inn as [?|inn]; [tauto | ].
+            specialize (IHe1i a); list_simpler; tauto.
+    Qed.
+
+    Corollary stratify_aux_free_vars
+          {e required_level bound_vars n sdefs} :
+      stratify_aux e required_level bound_vars = (n,sdefs) ->
+      incl (nnrc_free_vars e) bound_vars ->
+      equivlist (nnrc_free_vars n ++ (concat (map nnrc_free_vars (codomain sdefs)))) (nnrc_free_vars e ++ domain sdefs).
+    Proof.
+      apply stratify_aux_free_vars_and_growing.
+    Qed.
+
+    Corollary stratify_aux_free_vars_gfc
+          {e required_level bound_vars n sdefs} :
+      stratify_aux e required_level bound_vars = (n,sdefs) ->
+      incl (nnrc_free_vars e) bound_vars ->
+      growing_fv_ctxt sdefs (nnrc_free_vars e).
+    Proof.
+      apply stratify_aux_free_vars_and_growing.
+    Qed.
+    
+    Corollary stratify_aux_free_vars
+              {e required_level bound_vars n sdefs} :
+      stratify e required_level bound_vars = (n,sdefs) ->
+      incl (nnrc_free_vars e) bound_vars ->
+      equivlist (nnrc_free_vars n ++ (concat (map nnrc_free_vars (codomain sdefs)))) (nnrc_free_vars e ++ domain sdefs).
+    Proof.
+      apply stratify_aux_free_vars_and_growing.
+    Qed.
+
+  End FreeVars.
+  
+  Section Correct.
+
+    Opaque fresh_var.
+
+
+    Require Import cNNRCEq.
+
+    Lemma mk_expr_from_vars_binop b e1 e2 sdefs :
+      nnrc_core_eq
+        (mk_expr_from_vars (NNRCBinop b e1 e2, sdefs))
+        (NNRCBinop b (mk_expr_from_vars (e1, sdefs)) (mk_expr_from_vars (e2, sdefs))).
+    Proof.
+      unfold mk_expr_from_vars.
+      induction sdefs; simpl.
+      - reflexivity.
+      - rewrite IHsdefs; simpl.
+        red; simpl; intros.
+        match_case.
+    Qed.
+
+
+    Lemma stratify_aux_correct h cenv env e bound_vars required_kind :
+      incl (nnrc_free_vars e) bound_vars ->
+      Forall (data_normalized h) (map snd cenv) ->
+      Forall (data_normalized h) (map snd env) ->
+      @nnrc_core_eval _ h cenv env (mk_expr_from_vars (stratify_aux e required_kind bound_vars)) =
+      @nnrc_core_eval _ h cenv env e.
+    Proof.
+      revert required_kind bound_vars env.
+      induction e; intros required_kind bound_vars env fbincl Fde FDce; simpl; trivial.
+      - repeat (match_case; intros).
+        rewrite mk_expr_from_vars_binop; trivial.
+        simpl in *.
+        apply incl_app_iff in fbincl.
+        destruct fbincl as [fbincl1 fbincl2].
+        generalize (stratify_aux_nbound_vars H); intros nb1.
+        generalize (stratify_aux_nbound_vars H0); intros nb2.
+        specialize (IHe1 nnrcExpr bound_vars env).
+        cut_to IHe1; trivial.
+        rewrite H in IHe1.
+        rewrite <- IHe1.
+        specialize (IHe2 nnrcExpr (domain l ++ bound_vars) env).
+        cut_to IHe2; trivial; try (apply incl_appr; trivial).
+        rewrite H0 in IHe2.
+        rewrite <- IHe2.
+        repeat rewrite mk_expr_from_vars_app.
+        f_equal.
+        +
+    
+
+
+    Lemma mk_expr_from_vars_app e l1 l2 :
+      mk_expr_from_vars (e, (l1 ++ l2)) =
+      mk_expr_from_vars ((mk_expr_from_vars (e, l2)), l1).
+    Proof.
+      unfold mk_expr_from_vars; simpl.
+      rewrite fold_right_app.
+      trivial.
+    Qed.
+
+
+    
+
+
+
+    Lemma stratify_aux_free_vars {e required_level bound_vars n sdefs} :
+      incl (nnrc_free_vars e) bound_vars ->
+      stratify_aux e required_level bound_vars = (n,sdefs) ->
+      equivlist (nnrc_free_vars n ++ (concat (map nnrc_free_vars (codomain sdefs)))) (nnrc_free_vars e ++ domain sdefs).
+    Proof.
+      unfold equivlist.
+      revert required_level bound_vars sdefs n.
+      induction e; intros required_level bound_vars sdefs n inclb eqq
+      ; simpl in *; invcs eqq; simpl; unfold incl; try tauto.
+      - match_case_in H0; intros ? ? eqq1; rewrite eqq1 in H0.
+        match_case_in H0; intros ? ? eqq2; rewrite eqq2 in H0.
+        invcs H0; simpl.
+        apply incl_app_iff in inclb.
+        destruct inclb as [inclb1 inclb2].
+        specialize (IHe1 _ _ _ _ inclb1 eqq1).
+        assert (inclb2':incl (nnrc_free_vars e2) (domain l ++ bound_vars))
+               by (intros ? inn; list_simpler; intuition).
+        specialize (IHe2 _ _ _ _ inclb2' eqq2).
+        list_simpler.
+        intros a. specialize (IHe1 a); specialize (IHe2 a).
+        repeat rewrite in_app_iff in *.
+        intuition.
+      - admit.
+      - match_case_in H0; intros ? ? eqq1; rewrite eqq1 in H0.
+        apply incl_app_iff in inclb.
+        destruct inclb as [inclb1 inclb2].
+        specialize (IHe1 _ _ _ _ inclb1 eqq1).
+        destruct (stratify1_aux_sdefs_app H0) as [sdefs' ?]; subst.
+        case_eq (stratify_aux e2 nnrcStmt (v::bound_vars)); intros nn ll eqq2.
+        rewrite eqq2 in *.
+        assert (inclb2':incl (nnrc_free_vars e2) (v::bound_vars)).
+        { unfold incl in *; intros ? inn; simpl.
+          destruct (v == a); unfold equiv, complement in *.
+          - eauto.
+          - right; apply inclb2.
+            list_simpler; trivial.
+        } 
+        specialize (IHe2 _ _ _ _ inclb2' eqq2).
+        intros a.
+        specialize (IHe1 a); specialize (IHe2 a).
+        list_simpler.
+        split; intros inn.
+        * { intuition.
+              - generalize (stratify1_aux_free_vars_incl H0 _ H4); intros inn2.
+                simpl in inn2.
+                repeat rewrite domain_app in inn2.
+                repeat rewrite in_app_iff in inn2.
+                intuition.
+                list_simpler.
+                destruct required_level
+                ; simpl in H0; invcs H0
+                ; (repeat (list_simpler; simpl in *)); intuition.
+                   list_simpler.
+                   generalize (mk_expr_from_vars_growing_fv_free_fw_codomain H0); intros HH2.
+                   destruct HH2.
+                   + revert H1 H11; clear; intuition. apply H1 in H11.
+                     revert H11; clear; intuition.
+                   generalize (mk_expr_from_vars_growing_fv_free_fw gfc2 _ _ H0)
+                   ; intuition.
+             }
+
+                generalize (mk_expr_from_vars_growing_fv_free_fw gfc2 _ _ H3); intros HH.
+                intuition.
+              - destruct required_level
+                ; simpl in H0; invcs H0
+                ; (repeat (list_simpler; simpl in *)); intuition.
+                   list_simpler.
+                   generalize (mk_expr_from_vars_growing_fv_free_fw gfc2 _ _ H0)
+                   ; intuition.
+             }
+             * { 
+                 generalize (stratify_aux_nbound_vars eqq2); intros disj.
+                 apply disjoint_cons_inv2 in disj.
+                 destruct disj as [disj vnin].
+                 destruct required_level
+                ; simpl in H0; invcs H0
+                ; (repeat (list_simpler; simpl in *)); intuition; list_simpler.
+                   - specialize (H H2).
+                     generalize (mk_expr_from_vars_growing_fv_free_bk nn ll a)
+                     ; intros HH.
+                     specialize (inclb2' _ H2).
+                     simpl in inclb2'; destruct inclb2'; [congruence | ].
+                     symmetry in disj.
+                     specialize (disj _ H9).
+                     destruct H.
+                     + intuition.
+                     + generalize (mk_expr_from_vars_has_codomain_vars a ll)
+                       ; intuition.
+                   - specialize (H H2).
+                     generalize (mk_expr_from_vars_growing_fv_free_bk nn ll a)
+                     ; intros HH.
+                     specialize (inclb2' _ H2).
+                     simpl in inclb2'; destruct inclb2'; [congruence | ].
+                     symmetry in disj.
+                     specialize (disj _ H9).
+                     destruct H.
+                     + intuition.
+                     + generalize (mk_expr_from_vars_has_codomain_vars a ll)
+                       ; intuition.
+                    }
+          + rewrite growing_fv_ctxt_app; simpl; split.
+            * eapply growing_fv_ctxt_incl; eauto
+              ; intros ?; repeat rewrite in_app_iff; intuition.
+            * generalize (stratify1_aux_gfc_app_weak H0); intros HH.
+              simpl in HH.
+              { cut_to HH.
+                -
+                  generalize (mk_expr_from_vars_growing_fv_free_fw gfc1); intros HH2.
+                  eapply growing_fv_ctxt_incl; eauto
+                  ; intros ?; repeat rewrite in_app_iff; intuition.
+                  + specialize (incl1 a).
+                    list_simpler.
+                    intuition.
+                  + list_simpler.
+                    admit.
+                - eapply growing_fv_ctxt_incl; eauto
+                  ; intros ?; repeat rewrite in_app_iff; intuition.
+                  specialize (incl1 a).
+                  list_simpler.
+                  destruct incl1 as [incl11 incl12].
+                  cut_to incl12; [ | intuition].
+                  destruct incl12; [intuition | ].
+                  
+                  
+                  destruct required_level; simpl in H0.
+                  invcs H0.
+                ; simpl in H0; invcs H0
+                ; (repeat (list_simpler; simpl in *)).
+                  
+
+
+    Lemma stratify_aux_free_vars {e required_level bound_vars n sdefs} :
+      incl (nnrc_free_vars e) bound_vars ->
+      stratify_aux e required_level bound_vars = (n,sdefs) ->
+      (equivlist (nnrc_free_vars n ++ (concat (map nnrc_free_vars (codomain sdefs)))) (nnrc_free_vars e ++ domain sdefs)
+      /\ growing_fv_ctxt sdefs (nnrc_free_vars e)).
+    Proof.
+      unfold equivlist.
+      revert required_level bound_vars sdefs n.
+      induction e; intros required_level bound_vars sdefs n inclb eqq
+      ; simpl in *; invcs eqq; simpl; unfold incl; try tauto.
+      - match_case_in H0; intros ? ? eqq1; rewrite eqq1 in H0.
+        match_case_in H0; intros ? ? eqq2; rewrite eqq2 in H0.
+        invcs H0; simpl.
+        apply incl_app_iff in inclb.
+        destruct inclb as [inclb1 inclb2].
+        destruct (IHe1 _ _ _ _ inclb1 eqq1) as [incl1 gfc1].
+        assert (inclb2':incl (nnrc_free_vars e2) (domain l ++ bound_vars))
+               by (intros ? inn; list_simpler; intuition).
+        destruct (IHe2 _ _ _ _ inclb2' eqq2) as [incl2 gfc2].
+        list_simpler.
+        split.
+        + intros a. specialize (incl1 a); specialize (incl2 a).
+          repeat rewrite in_app_iff in *.
+          intuition.
+        + rewrite growing_fv_ctxt_app; simpl; split.
+          * eapply growing_fv_ctxt_incl; eauto
+            ; intros ?; repeat rewrite in_app_iff; intuition.
+          * eapply growing_fv_ctxt_incl; eauto
+            ; intros ?; repeat rewrite in_app_iff; intuition.
+      - admit.
+      - match_case_in H0; intros ? ? eqq1; rewrite eqq1 in H0.
+        apply incl_app_iff in inclb.
+        destruct inclb as [inclb1 inclb2].
+        destruct (IHe1 _ _ _ _ inclb1 eqq1) as [incl1 gfc1].
+        destruct (stratify1_aux_sdefs_app H0) as [sdefs' ?]; subst.
+        case_eq (stratify_aux e2 nnrcStmt (v::bound_vars)); intros nn ll eqq2.
+        rewrite eqq2 in *.
+        assert (inclb2':incl (nnrc_free_vars e2) (v::bound_vars)).
+        { unfold incl in *; intros ? inn; simpl.
+          destruct (v == a); unfold equiv, complement in *.
+          - eauto.
+          - right; apply inclb2.
+            list_simpler; trivial.
+        } 
+        specialize (IHe2 _ _ _ _ inclb2' eqq2).
+        destruct IHe2 as [incl2 gfc2].
+        split.
+        + intros a.
+          specialize (incl1 a); specialize (incl2 a).
+          list_simpler.
+          split; intros inn.
+          * { intuition.
+              - generalize (stratify1_aux_free_vars_incl H0 _ H4); intros inn2.
+                simpl in inn2.
+                repeat rewrite domain_app in inn2.
+                repeat rewrite in_app_iff in inn2.
+                intuition.
+                list_simpler.
+                generalize (mk_expr_from_vars_growing_fv_free_fw gfc2 _ _ H3); intros HH.
+                intuition.
+              - destruct required_level
+                ; simpl in H0; invcs H0
+                ; (repeat (list_simpler; simpl in *)); intuition.
+                   list_simpler.
+                   generalize (mk_expr_from_vars_growing_fv_free_fw gfc2 _ _ H0)
+                   ; intuition.
+             }
+             * { 
+                 generalize (stratify_aux_nbound_vars eqq2); intros disj.
+                 apply disjoint_cons_inv2 in disj.
+                 destruct disj as [disj vnin].
+                 destruct required_level
+                ; simpl in H0; invcs H0
+                ; (repeat (list_simpler; simpl in *)); intuition; list_simpler.
+                   - specialize (H H2).
+                     generalize (mk_expr_from_vars_growing_fv_free_bk nn ll a)
+                     ; intros HH.
+                     specialize (inclb2' _ H2).
+                     simpl in inclb2'; destruct inclb2'; [congruence | ].
+                     symmetry in disj.
+                     specialize (disj _ H9).
+                     destruct H.
+                     + intuition.
+                     + generalize (mk_expr_from_vars_has_codomain_vars a ll)
+                       ; intuition.
+                   - specialize (H H2).
+                     generalize (mk_expr_from_vars_growing_fv_free_bk nn ll a)
+                     ; intros HH.
+                     specialize (inclb2' _ H2).
+                     simpl in inclb2'; destruct inclb2'; [congruence | ].
+                     symmetry in disj.
+                     specialize (disj _ H9).
+                     destruct H.
+                     + intuition.
+                     + generalize (mk_expr_from_vars_has_codomain_vars a ll)
+                       ; intuition.
+                    }
+          + rewrite growing_fv_ctxt_app; simpl; split.
+            * eapply growing_fv_ctxt_incl; eauto
+              ; intros ?; repeat rewrite in_app_iff; intuition.
+            * generalize (stratify1_aux_gfc_app_weak H0); intros HH.
+              simpl in HH.
+              { cut_to HH.
+                -
+                  generalize (mk_expr_from_vars_growing_fv_free_fw gfc1); intros HH2.
+                  eapply growing_fv_ctxt_incl; eauto
+                  ; intros ?; repeat rewrite in_app_iff; intuition.
+                  + specialize (incl1 a).
+                    list_simpler.
+                    intuition.
+                  + list_simpler.
+                    admit.
+                - eapply growing_fv_ctxt_incl; eauto
+                  ; intros ?; repeat rewrite in_app_iff; intuition.
+                  specialize (incl1 a).
+                  list_simpler.
+                  destruct incl1 as [incl11 incl12].
+                  cut_to incl12; [ | intuition].
+                  destruct incl12; [intuition | ].
+                  
+                  
+                  destruct required_level; simpl in H0.
+                  invcs H0.
+                ; simpl in H0; invcs H0
+                ; (repeat (list_simpler; simpl in *)).
+                  
+                 
+            
+
+                 
+    
+    Lemma stratify_aux_free_vars {e required_level bound_vars n sdefs} :
+      stratify_aux e required_level bound_vars = (n,sdefs) ->
+      (incl (nnrc_free_vars n) (nnrc_free_vars e ++ domain sdefs)
+      /\ growing_fv_ctxt sdefs (nnrc_free_vars e)).
+    Proof.
+      unfold incl.
+      revert required_level bound_vars sdefs n.
+      induction e; intros required_level bound_vars sdefs n eqq
+      ; simpl in *; invcs eqq; simpl; unfold incl; try tauto.
+      - match_case_in H0; intros ? ? eqq1; rewrite eqq1 in H0.
+        match_case_in H0; intros ? ? eqq2; rewrite eqq2 in H0.
+        invcs H0; simpl.
+        destruct (IHe1 _ _ _ _ eqq1) as [incl1 gfc1].
+        destruct (IHe2 _ _ _ _ eqq2) as [incl2 gfc2].
+        repeat rewrite domain_app in *.
+        split.
+        + intros a inn. specialize (incl1 a); specialize (incl2 a).
+          repeat rewrite in_app_iff in *.
+          intuition.
+        + rewrite growing_fv_ctxt_app; simpl; split.
+          * eapply growing_fv_ctxt_incl; eauto
+            ; intros ?; repeat rewrite in_app_iff; intuition.
+          * eapply growing_fv_ctxt_incl; eauto
+            ; intros ?; repeat rewrite in_app_iff; intuition.
+      - admit.
+      - match_case_in H0; intros ? ? eqq1; rewrite eqq1 in H0.
+        destruct (IHe1 _ _ _ _ eqq1) as [incl1 gfc1].
+        destruct (stratify1_aux_sdefs_app H0) as [sdefs' ?]; subst.
+        case_eq (stratify_aux e2 nnrcStmt bound_vars); intros nn ll eqq2.
+        rewrite eqq2 in *.
+        specialize (IHe2 _ _ _ _ eqq2).
+        destruct IHe2 as [incl2 gfc2].
+        split.
+        + intros ? inn.
+          generalize (stratify1_aux_free_vars_incl H0 _ inn); intros inn2.
+          simpl in inn2.
+          specialize (incl1 a).
+          repeat rewrite domain_app in *.
+          repeat rewrite in_app_iff in *.
+          intuition.
+          apply remove_inv in H1.
+          destruct H1 as [inn2 neq].
+          rewrite <- (remove_in_neq _ _ _ neq).
+          generalize (mk_expr_from_vars_growing_fv_free_fw gfc2 _ _ inn2); intros HH.
+          specialize (incl2 a).
+          repeat rewrite in_app_iff in *; intuition.
+        + rewrite growing_fv_ctxt_app; simpl; split.
+          * eapply growing_fv_ctxt_incl; eauto
+            ; intros ?; repeat rewrite in_app_iff; intuition.
+          * generalize (stratify1_aux_gfc_app_weak H0); intros HH.
+            simpl in HH.
+            { cut_to HH.
+              - admit.
+              -  eapply growing_fv_ctxt_incl; eauto
+                 ; intros ?; repeat rewrite in_app_iff; intuition.
+                 
+            
+            
+          * eapply growing_fv_ctxt_incl; eauto
+            ; intros ?; repeat rewrite in_app_iff; intuition.
+          * 
+            eapply growing_fv_ctxt_incl; eauto
+            ; intros ?; repeat rewrite in_app_iff; intuition.
+
+    Qed.
+            
+    Lemma stratify_aux_growing_fv_ctxt {e required_level bound_vars n sdefs} :
+      stratify_aux e required_level bound_vars = (n,sdefs) ->
+      growing_fv_ctxt sdefs (nnrc_free_vars e).
+    Proof.
+      revert required_level bound_vars sdefs n.
+      induction e; intros required_level bound_vars sdefs n eqq
+      ; simpl in *; invcs eqq; simpl; trivial.
+      - match_case_in H0; intros ? ? eqq1; rewrite eqq1 in H0.
+        match_case_in H0; intros ? ? eqq2; rewrite eqq2 in H0.
+        invcs  H0.
+        apply growing_fv_ctxt_app.
+        apply IHe1 in eqq1.
+        apply IHe2 in eqq2.
+        split.
+        + eapply growing_fv_ctxt_incl; eauto; intro; rewrite in_app_iff; intuition.
+        + eapply growing_fv_ctxt_incl; eauto; intro; rewrite in_app_iff; intuition.
+      - admit.
+      - match_case_in H0; intros ? ? eqq1; rewrite eqq1 in H0.
+        specialize (IHe1 _ _ _ _ eqq1).
+        destruct required_level; simpl in H0; invcs H0.
+        + apply growing_fv_ctxt_app.
+          split.
+          * eapply growing_fv_ctxt_incl; eauto; intro; rewrite in_app_iff; intuition.
+          * simpl.
+            generalize (mk_expr_from_vars_growing_fv_free_fw IHe1); intros HH.
+            split; trivial.
+            intros ? inn.
+            repeat rewrite in_app_iff in *.
+            
+            
+            
+        match_case_in H0; intros ? ? eqq2; rewrite eqq2 in H0.
+
+        
+
+
+    Lemma mk_expr_from_vars_growing_fv_free e sdefs ctxt :
+      disjoint (domain sdefs) (ctxt++nnrc_free_vars e) ->
+      growing_fv_ctxt sdefs (ctxt++(nnrc_free_vars e)) ->
+      forall x,
+        In x (ctxt++nnrc_free_vars (mk_expr_from_vars (e, sdefs))) <->
+        ((In x (ctxt++(nnrc_free_vars e))) /\ ~ In x (domain sdefs)).
+    Proof.
+      unfold mk_expr_from_vars.
+      revert e ctxt; induction sdefs; intros e ctxt disj gfc; simpl; [intuition | ].
+      intros; destruct a; simpl in *.
+      destruct gfc as [incln gfc].
+      apply disjoint_cons_inv1 in disj.
+      destruct disj as [disj nin].
+      repeat rewrite in_app_iff in *.
+      split; intros inn.
+      - destruct inn as [inn|[inn|inn]]; [intuition | .. ].
+        + subst; intuition.
+        + eapply disj; eauto.
+          rewrite in_app_iff; eauto.
+        + intuition; subst.
+          * apply incln in inn.
+            rewrite in_app_iff in inn; intuition.
+          * apply incln in inn.
+            eapply disj; eauto.
+        + apply remove_inv in inn.
+          destruct inn as [inn neq].
+          
+          
+      - subst; intuition.
+      - admit.
+      - admit.
+      - admit.
+      - apply remove_inv in H.
+        destruct H as [inn neq].
+        rewrite mk_expr_from_vars_eq in *.
+        admit.
+      - apply remove_inv in H.
+        destruct H as [inn neq].
+        rewrite mk_expr_from_vars_eq in *.
+        admit.
+        
+        
+
+    Lemma mk_expr_from_vars_preserves_same_free e sdefs :
+          (forall x y, In (x,y) sdefs -> incl (nnrc_free_vars y) (nnrc_free_vars e)) ->
+          incl (nnrc_free_vars (mk_expr_from_vars (e, sdefs)))
+               (nnrc_free_vars e).
+    Proof.
+      unfold mk_expr_from_vars.
+      induction sdefs; simpl; intros incls; [reflexivity | ].
+      red; intros ? inn.
+      rewrite in_app_iff in inn.
+      destruct inn as [inn|inn].
+      - specialize (incls (fst a) (snd a)).
+        destruct a; simpl in *.
+        intuition.
+      - apply remove_inv in inn.
+        destruct inn as [inn Hneq].
+        apply IHsdefs in inn; trivial.
+        eauto.
+    Qed.
+
+    (* critical condition *)
+    Lemma stratify1_aux_correct h cenv env e bound_vars required_kind sdefs :
+      incl (nnrc_free_vars e) bound_vars ->
+      disjoint bound_vars (domain sdefs) ->
+      (forall x y, In (x,y) sdefs -> incl (nnrc_free_vars y) (nnrc_free_vars e)) ->
+      @nnrc_core_eval _ h cenv env (mk_expr_from_vars (stratify1_aux e required_kind bound_vars sdefs)) =
+      @nnrc_core_eval _ h cenv env (mk_expr_from_vars (e,sdefs)).
+    Proof.
+      destruct required_kind; simpl; trivial.
+      unfold mk_expr_from_vars; simpl.
+      rewrite fold_right_app; simpl.
+      revert e.
+      induction sdefs; simpl; intros e inbfv disj same_free.
+      - match_option.
+        match_destr; try congruence.
+      - match_option.
+        specialize (IHsdefs e).
+        repeat rewrite mk_expr_from_vars_eq in *.
+        generalize (@cNNRCShadow.nnrc_core_eval_remove_free_env _ h cenv
+                                                                nil); simpl; intros HH.
+        repeat rewrite HH.
+        + apply IHsdefs; intuition.
+          * apply disjoint_cons_inv2 in disj.
+            intuition.
+          * eapply same_free; right; eauto.
+        + intro inn.
+          apply mk_expr_from_vars_preserves_same_free in inn.
+          * apply inbfv in inn.
+            apply disjoint_cons_inv2 in disj.
+            intuition.
+          * intuition; eauto.
+        + intro inn.
+          apply mk_expr_from_vars_preserves_same_free in inn.
+          * simpl in inn.
+            match_destr_in inn; try congruence.
+            rewrite app_nil_r in inn.
+            apply inbfv in inn.
+            apply disjoint_cons_inv2 in disj.
+            intuition.
+          * intros ? ? inn2.
+            simpl; match_destr; try congruence.
+            rewrite app_nil_r.
+            eapply same_free; eauto.
+    Qed.
+
+
+
+
+
+    (*
+
+    Lemma stratify1_aux_free_vars {e required_kind bound_vars sdefs n l} :
+      stratify1_aux e required_kind bound_vars sdefs = (n,l) ->
+      bound_vars ++ (domain sdefs)
+      equivlist (nnrc_free_vars e ++ domain sdefs) (nnrc_free_vars n ++ domain l).
+    Proof.
+      destruct required_kind; simpl; trivial; intros eqq; invcs eqq; simpl; trivial.
+      - rewrite domain_app.
+      - reflexivity.
+      intros.
+      rewrite domain_app, in_app_iff in inn.
+      destruct inn; trivial.
+      - simpl in *.
+        destruct H0; try tauto.
+        subst.
+        apply fresh_var_fresh in H.
+        tauto.
+
+    Qed.
+      
+    Lemma stratify_aux_free_vars {e required_kind bound_vars n l} :
+      stratify_aux e required_kind bound_vars = (n,l) ->
+      equivlist (nnrc_free_vars n) (nnrc_free_vars e ++ domain l).
+*)
+
+
+
+
+
+
+    Lemma stratify_aux_free_vars_incl {fe n sdefs} :
+      incl (nnrc_free_vars n) (fe ++ (domain sdefs)) ->
+      (forall x y, In (x,y) sdefs -> incl (nnrc_free_vars y) fe) ->
+      incl (nnrc_free_vars (mk_expr_from_vars (n,sdefs))) fe.
+    Proof.
+      unfold mk_expr_from_vars.
+      revert fe n.
+      induction sdefs; intros fe n incl1 incl2; simpl in *.
+      - rewrite app_nil_r in incl1; trivial.
+      - intros ? inn.
+        rewrite in_app_iff in inn.
+        destruct inn as [inn|inn].
+        + destruct a as [aa ab].
+          specialize (incl2 aa ab); intuition.
+        + apply remove_inv in inn.
+          destruct inn as [inn neq].
+          eapply IHsdefs; try eapply inn; eauto.
+          intros ? inn2.
+          specialize (incl1 _ inn2).
+          rewrite in_app_iff in incl1; simpl in incl1.
+          rewrite in_app_iff.
+          intuition.
+          subst.
+          
+
+          
+    In a (nnrc_free_vars (mk_expr_from_vars (stratify_aux e nnrcStmt bound_vars))) = nnrc_free_vars e
+
+    
+    Lemma stratify_aux_free_vars_incl {e required_level bound_vars n sdefs} :
+      stratify_aux e required_level bound_vars = (n, sdefs) ->
+      (incl (nnrc_free_vars n) (nnrc_free_vars e ++ (domain sdefs))
+    /\ (forall x y, In (x,y) sdefs -> incl (nnrc_free_vars y) (nnrc_free_vars e))).
+    Proof.
+      revert required_level bound_vars sdefs n.
+      induction e; intros required_level bound_vars sdefs n eqq
+      ; simpl in *; invcs eqq; simpl.
+      - intuition.
+      - intuition.
+      - intuition.
+      - match_case_in H0; intros ? ? eqq1
+        ; rewrite eqq1 in H0.
+         match_case_in H0; intros ? ? eqq2
+         ; rewrite eqq2 in H0.
+         invcs H0; simpl.
+         destruct (IHe1 _ _ _ _ eqq1) as [IHe11 IHe12].
+         destruct (IHe2 _ _ _ _ eqq2) as [IHe21 IHe22].
+         split
+         ; unfold incl in *; [intros ? inn | intros ? ? inn1 ? inn2]
+          ; repeat rewrite domain_app in *
+          ; repeat rewrite in_app_iff in *.
+        + destruct inn as [inn|inn].
+          * specialize (IHe11 _ inn).
+            rewrite in_app_iff in IHe11.
+            intuition.
+          * specialize (IHe21 _ inn).
+            rewrite in_app_iff in IHe21.
+            intuition.
+        + intuition eauto.
+      -  match_case_in H0; intros ? ? eqq1
+         ; rewrite eqq1 in H0.
+         invcs H0; simpl.
+         eauto.
+      - match_case_in H0; intros ? ? eqq1
+        ; rewrite eqq1 in H0; simpl.
+        specialize (IHe1 _ _ _ _ eqq1).
+        destruct IHe1 as [IHe11 IHe12].
+        destruct (stratify1_aux_sdefs_app H0); subst.
+        apply stratify1_aux_free_vars_incl in H0.
+        simpl in H0.
+        split; [intros ? inn | intros ? ? inn1 ? inn2]
+        ; repeat rewrite domain_app
+        ; repeat rewrite in_app_iff.
+        + specialize (H0 _ inn).
+          rewrite domain_app in H0.
+          repeat rewrite in_app_iff in H0.
+          intuition.
+          * specialize (IHe11 _ H0).
+            rewrite in_app_iff in IHe11.
+            intuition.
+          *  apply remove_inv in H0.
+             destruct H0 as [inn2 neq].
+             rewrite <- remove_in_neq by trivial.
+
+
+             case_eq ((stratify_aux e2 nnrcStmt bound_vars)); intros ? ? eqq2
+             ; rewrite eqq2 in *.
+             specialize (IHe2 _ _ _ _ eqq2).
+             destruct IHe2 as [IHe21 IHe22].
+             
+             
+             specialize (mk_expr_from_vars_preserves_same_free n1 l0)
+             ; intros incl2.
+             { cut_to incl2.
+               - admit.
+               - intros ? ? inn3 ? inn4.
+                 specialize (IHe22 _ _ inn3 _ inn4).
+             
+             
+          
+          generalize (
+          
+SearchAbout remove.
+          
+
+          
+          
+          generalize (mk_expr_from_vars_preserves_same_free 
+          
+              
+        specialize (stratify1_aux_nbound_vars H0); intros HH.
+        eapply disjoint_with_exclusion; eauto.
+      - match_case_in H0; intros ? ? eqq1
+        ; rewrite eqq1 in H0.
+        specialize (IHe1 _ _ _ _ eqq1).
+        specialize (stratify1_aux_nbound_vars H0); intros HH.
+        eapply disjoint_with_exclusion; eauto.
+      - match_case_in H0; intros ? ? eqq1
+        ; rewrite eqq1 in H0.
+        specialize (IHe1 _ _ _ _ eqq1).
+        specialize (stratify1_aux_nbound_vars H0); intros HH.
+        eapply disjoint_with_exclusion; eauto.
+      - match_case_in H0; intros ? ? eqq1
+        ; rewrite eqq1 in H0.
+        specialize (IHe1 _ _ _ _ eqq1).
+        specialize (stratify1_aux_nbound_vars H0); intros HH.
+        eapply disjoint_with_exclusion; eauto.
+      - match_case_in H0; intros ? ? eqq1
+         ; rewrite eqq1 in H0.
+         invcs H0.
+         eauto.
+    Qed.
+    Lemma stratify_aux_correct h cenv env e bound_vars required_kind :
+      incl (nnrc_free_vars e) bound_vars ->
+      Forall (data_normalized h) (map snd cenv) ->
+      Forall (data_normalized h) (map snd env) ->
+      @nnrc_core_eval _ h cenv env (mk_expr_from_vars (stratify_aux e required_kind bound_vars)) =
+      @nnrc_core_eval _ h cenv env e.
+    Proof.
+      revert required_kind bound_vars env.
+      induction e; intros required_kind bound_vars env fbincl Fde FDce; simpl; trivial.
+      - repeat (match_case; intros).
+        rewrite mk_expr_from_vars_binop; trivial.
+        simpl in *.
+        apply incl_app_iff in fbincl.
+        destruct fbincl as [fbincl1 fbincl2].
+        generalize (stratify_aux_nbound_vars H); intros nb1.
+        generalize (stratify_aux_nbound_vars H0); intros nb2.
+        specialize (IHe1 nnrcExpr bound_vars env).
+        cut_to IHe1; trivial.
+        rewrite H in IHe1.
+        rewrite <- IHe1.
+        specialize (IHe2 nnrcExpr (domain l ++ bound_vars) env).
+        cut_to IHe2; trivial; try (apply incl_appr; trivial).
+        rewrite H0 in IHe2.
+        rewrite <- IHe2.
+        repeat rewrite mk_expr_from_vars_app.
+        f_equal.
+        +
+
+          
+
+
+          
+          
+        + 
+
+          
+          
+        + 
+        
+        SearchAbout fold_right.
+            Definition mk_expr_from_vars (nws:nnrc_with_substs)
+      := fold_right (fun sdef accum => NNRCLet (fst sdef) (snd sdef) accum) (fst nws) (snd nws).
+
+      - 
+
+        Lemma nnrc_core_eval_remove_free_env {h:list (string*string)} c l v x l' e :
+          disjoint (domain l3) (nnrc_free_vars e) ->
+          nnrc_core_eval h c (l ++ l3 ++ l') e = nnrc_core_eval h c (l ++ l') e.
+  Proof.
+
+        
+        
+        rewrite IHe1.
+        
+        
+        rewrite IHe1.
+        
+
+
+      
+    Section tests.
+    Local Open Scope nnrc_scope.
+    Local Open Scope string_scope.
+
+    Eval vm_compute in (stratify nnrc1).
+
+    Eval vm_compute in (stratify nnrc2).
+    Eval vm_compute in (stratify nnrc2).
+
+    Example nnrcC1 := (NNRCFor "x"%string ‵(dnat 1) ‵(dnat 2)) ‵+ (NNRCFor "y"%string ‵(dnat 3) ‵(dnat 4)).
+    Eval vm_compute in (stratify nnrcC1).
+    
+(*    Example nnrc3 := (‵abs (NNRCLet "x" ((‵(dnat 1) ‵+ ‵(dnat 2))) (((NNRCVar "x" ‵+ ‵(dnat 8)))) ‵+ ‵(dnat 5)) ‵+ ((‵(dnat 4) ‵+ ‵(dnat 7)) ‵+‵`(dnat  3))). *)
+    Eval vm_compute in (stratify nnrc3). 
+
+    Example nnrc4 := (‵abs (NNRCFor "x" ((‵(dnat 1) ‵+ ‵(dnat 2))) (((NNRCVar "x" ‵+ ‵(dnat 8)))) ‵+ ‵(dnat 5)) ‵+ ((‵(dnat 4) ‵+ ‵(dnat 7)) ‵+‵`(dnat  3))).
+(*    Eval vm_compute in (stratify nnrc4). *)
+
+    Example nnrc5 := (‵abs (NNRCLet "z" (NNRCFor "x" ((‵(dnat 1) ‵+ ‵(dnat 2))) (((NNRCVar "x" ‵+ ‵(dnat 8)))) ‵+ ‵(dnat 5)) (NNRCVar "z")) ‵+ ((‵(dnat 4) ‵+ ‵(dnat 7)) ‵+‵`(dnat  3))).
+(*    Eval vm_compute in (stratify nnrc5). *)
+
+    Example nnrc6 := (‵abs (NNRCLet "z" (NNRCFor "x" ((‵(dnat 1) ‵+ ‵(dnat 2))) (((NNRCVar "x" ‵+ ‵(dnat 8))))) (NNRCVar "z")) ‵+ ((‵(dnat 4) ‵+ ‵(dnat 7)) ‵+‵`(dnat  3))).
+(*    Eval vm_compute in (stratify nnrc6). *)
+
+    Example nnrc7 := NNRCLet "x" (NNRCLet "y" ‵(dnat 3) (‵(dnat 8) ‵+ (NNRCVar "y"))) (NNRCVar "x").
+    
+(*    Eval vm_compute in (stratify nnrc7). *)
+
+    Example nnrc8 := NNRCLet "x" (NNRCLet "x" ‵(dnat 3) (‵(dnat 8) ‵+ (NNRCVar "x"))) (NNRCVar "x").
+    
+(*    Eval vm_compute in (stratify nnrc8). *)
+
+  End tests.
+        Definition stratify1_aux
+               (body:nnrc)
+               (required_kind:nnrcKind)
+               (bound_vars:list var)
+               (sdefs:list (var*nnrc))
+      : nnrc_with_substs
+      := match required_kind with
+         | nnrcExpr =>
+           let fvar := fresh_var "stratify" bound_vars in
+           (NNRCVar fvar, (fvar, body)::sdefs)
+         | _ => (body, sdefs)
+         end.
+    
+    Fixpoint stratify_aux (e: nnrc) (required_kind:nnrcKind) (bound_vars:list var): nnrc_with_substs
+      := match e with
+         | NNRCG
+                    
+    
+         
+
+
+
+
+
+        Definition stratify1_aux
                (body:nnrc)
                (required_kind:nnrcKind)
                (bindings:list var)
@@ -281,277 +2269,217 @@ Section Stratify.
                            stratify1_aux body required_kind bound_vars1 holey_expr)
          end.
 
-    Definition stratify (e: nnrc) : nnrc
-      := stratify_aux e nnrcStmt nil (fun e _ => e).
+    (*
+    Definition holey_preserver
+               h cenv (holey_expr:nnrc->list var -> nnrc) 
+      := forall moreenv e e' env,
+        Forall (data_normalized h) (map snd env) ->
+        Forall (data_normalized h) (map snd moreenv) ->
+        incl (nnrc_free_vars e) (domain env) ->
+        nnrc_core_eval h cenv env e = nnrc_core_eval h cenv env e' ->
+        disjoint moreenv env ->
+        nnrc_core_eval h cenv (moreenv++env) (holey_expr e (domain env))
+        = nnrc_core_eval h cenv (moreenv++env) (holey_expr e' (domain moreenv++(domain env))).
+*)
 
-  End stratify.
-  Section tests.
-    Local Open Scope nnrc_scope.
-    Local Open Scope string_scope.
-
-    Example nnrc1 := (‵abs ‵ (dnat 3) ‵+ ‵(dnat 5)) ‵+ ((‵(dnat 4) ‵+ ‵(dnat 7)) ‵+‵`(dnat  3)).
-(*    Eval vm_compute in (stratify nnrc1). *)
-
-    Example nnrc2 := NNRCLet "x" nnrc1 (NNRCVar "x").
-(*    Eval vm_compute in (stratify nnrc2). *)
-
-    Example nnrc3 := (‵abs (NNRCLet "x" ((‵(dnat 1) ‵+ ‵(dnat 2))) (((NNRCVar "x" ‵+ ‵(dnat 8)))) ‵+ ‵(dnat 5)) ‵+ ((‵(dnat 4) ‵+ ‵(dnat 7)) ‵+‵`(dnat  3))).
-(*    Eval vm_compute in (stratify nnrc3). *)
-
-    Example nnrc4 := (‵abs (NNRCFor "x" ((‵(dnat 1) ‵+ ‵(dnat 2))) (((NNRCVar "x" ‵+ ‵(dnat 8)))) ‵+ ‵(dnat 5)) ‵+ ((‵(dnat 4) ‵+ ‵(dnat 7)) ‵+‵`(dnat  3))).
-(*    Eval vm_compute in (stratify nnrc4). *)
-
-    Example nnrc5 := (‵abs (NNRCLet "z" (NNRCFor "x" ((‵(dnat 1) ‵+ ‵(dnat 2))) (((NNRCVar "x" ‵+ ‵(dnat 8)))) ‵+ ‵(dnat 5)) (NNRCVar "z")) ‵+ ((‵(dnat 4) ‵+ ‵(dnat 7)) ‵+‵`(dnat  3))).
-(*    Eval vm_compute in (stratify nnrc5). *)
-
-    Example nnrc6 := (‵abs (NNRCLet "z" (NNRCFor "x" ((‵(dnat 1) ‵+ ‵(dnat 2))) (((NNRCVar "x" ‵+ ‵(dnat 8))))) (NNRCVar "z")) ‵+ ((‵(dnat 4) ‵+ ‵(dnat 7)) ‵+‵`(dnat  3))).
-(*    Eval vm_compute in (stratify nnrc6). *)
-
-    Example nnrc7 := NNRCLet "x" (NNRCLet "y" ‵(dnat 3) (‵(dnat 8) ‵+ (NNRCVar "y"))) (NNRCVar "x").
+    Inductive holey_some_preserver h cenv : (nnrc->list var -> nnrc) -> Prop
+      :=
+      | holey_some_preserver_base holey_expr v d e env :
+           Forall (data_normalized h) (map snd env) ->
+           incl (nnrc_free_vars e) (domain env) ->
+           ~ In v (domain env) ->
+           nnrc_core_eval h cenv env e = Some d ->
+           nnrc_core_eval h cenv env (holey_expr e (domain env))
+           = nnrc_core_eval h cenv ((v,d)::env) (holey_expr (NNRCVar v) (v::(domain env))) -> holey_some_preserver h cenv holey_expr
+      | holey_some_preserver_ind
+          holey_expr
+    .
     
-(*    Eval vm_compute in (stratify nnrc7). *)
-
-    Example nnrc8 := NNRCLet "x" (NNRCLet "x" ‵(dnat 3) (‵(dnat 8) ‵+ (NNRCVar "x"))) (NNRCVar "x").
-    
-(*    Eval vm_compute in (stratify nnrc8). *)
-
-  End tests.
-
-  Section Effective.
-
-    Lemma stratify1_aux_stratified body required_level hb holey_expr :
-      (forall (he : nnrc) (hb : list var),
-          stratifiedLevel required_level he -> stratified (holey_expr he hb)) ->
-      stratifiedLevel nnrcStmt body ->
-      stratified (stratify1_aux body required_level hb holey_expr).
-    Proof.
-      unfold stratified, stratify1_aux.
-      intros hpf ab.
-      destruct required_level; simpl; intuition.
-      apply hpf; simpl; trivial.
-    Qed.
-    
-    Lemma stratify_aux_stratified
-          (e: nnrc)
-          (required_level:nnrcKind)
-          (bindings:list var)
-          (holey_expr:nnrc->list var->nnrc) :
-      (forall he hb,
-          stratifiedLevel required_level he ->
-          stratified (holey_expr he hb)) ->
-      stratified (stratify_aux e required_level bindings holey_expr).
-    Proof.
-      unfold stratified.
-      revert required_level bindings holey_expr.
-      induction e; intros required_level bindings holey_expr holey_stratify; simpl;
-        repeat ((first [
-                     apply holey_stratify
-                   | apply IHe
-                   | apply IHe1
-                   | apply IHe2
-                   | apply IHe3
-                   | apply stratify1_aux_stratified
-                ]); simpl; intuition).
-    Qed.
-
-    Theorem stratify_stratified (e: nnrc) : stratified (stratify e).
-    Proof.
-      apply stratify_aux_stratified; intros.
-      apply stratifiedLevel_stratified in H; trivial.
-    Qed.
-
-    Corollary stratify_stratified_spec (e: nnrc) : stratified_spec (stratify e).
-    Proof.
-      apply stratified_correct.
-      apply stratify_stratified.
-    Qed.
-
-  End Effective.
-
-  Section Idempotent.
-    
-    Lemma stratify_aux_stratify_id
-          (e: nnrc)
-          (required_level:nnrcKind)
-          (bindings:list var)
-          (holey_expr:nnrc->list var->nnrc) :
-      stratifiedLevel required_level e ->              
-      stratify_aux e required_level bindings holey_expr = holey_expr e bindings.
-    Proof.
-      revert holey_expr bindings required_level.
-      induction e; intros holey_expr bindings required_level stratifylevc
-      ; repeat (simpl in *; intuition; subst; first [
-                                                  rewrite IHe
-                                                | rewrite IHe1
-                                                | rewrite IHe2
-                                                | rewrite IHe3]
-               ).
-    Qed.
-
-    Theorem stratify_stratify_id (e: nnrc) :
-      stratified e ->              
-      stratify e = e.
-    Proof.
-      intros stratifye.
-      apply stratify_aux_stratify_id.
-      apply stratifye.
-    Qed.
-
-    Corollary stratify_idem (e: nnrc) :
-      stratify (stratify e) = stratify e.
-    Proof.
-      apply stratify_stratify_id.
-      apply stratify_stratified.
-    Qed.
-
-  End Idempotent.
-
-  Section Correct.
-    
-    Definition holey_bindings_equiv (holey_expr:nnrc->list var->nnrc) :=
-      Proper (eq ==> equivlist ==> eq) holey_expr.
-
-    Lemma stratify1_aux_ext e required_level bindings holey_expr1 holey_expr2 :
-      (forall e b, holey_expr1 e b = holey_expr2 e b) ->
-      stratify1_aux e required_level bindings holey_expr1 = stratify1_aux e required_level bindings holey_expr2.
-    Proof.
-      intros; unfold stratify1_aux.
-      destruct required_level; congruence.
-    Qed.
-    
-    Lemma stratify_aux_ext e required_level bindings holey_expr1 holey_expr2 :
-      (forall e b, holey_expr1 e b = holey_expr2 e b) ->
-      stratify_aux e required_level bindings holey_expr1 = stratify_aux e required_level bindings holey_expr2.
-    Proof.
-      revert required_level bindings holey_expr1 holey_expr2.
-      induction e; intros required_level bindings holey_expr1 holey_expr2 ext; simpl; auto 3;
-        try solve [((apply IHe1 || apply IHe); intros; (apply stratify1_aux_ext || f_equal); auto)].
-    Qed.
-
-    
-    Lemma holey_bindings_stratify1_aux_equiv e required_level bindings1 bindings2 holey_expr :
-      Proper (eq ==> equivlist ==> eq) holey_expr ->
-      equivlist bindings1 bindings2 ->
-      stratify1_aux e required_level bindings1 holey_expr = stratify1_aux e required_level bindings2 holey_expr.
-    Proof.
-      intros.
-      unfold stratify1_aux.
-      destruct required_level; trivial.
-      - assert (fveq:fresh_var "stratify" bindings1 = fresh_var "stratify" bindings2) by (rewrite H0; reflexivity).
-        repeat rewrite fveq.
-        f_equal; trivial.
-        apply H; trivial.
-        apply equivlist_cons; trivial.
-      - rewrite H0; trivial.
-    Qed.
-
-    Lemma stratify1_aux_proper e1 e2 required_level bindings1 bindings2 holey_expr1 holey_expr2 :
-      e1 = e2 ->
-      Proper (eq ==> equivlist ==> eq) holey_expr1 ->
-      equivlist bindings1 bindings2 ->
-      (forall e b, holey_expr1 e b = holey_expr2 e b) ->
-      stratify1_aux e1 required_level bindings1 holey_expr1 = stratify1_aux e2 required_level bindings2 holey_expr2.
-    Proof.
-      intros; subst.
-      transitivity (stratify1_aux e2 required_level bindings2 holey_expr1).
-      - apply holey_bindings_stratify1_aux_equiv; trivial.
-      - apply stratify1_aux_ext; trivial.
-    Qed.
-
-    Lemma holey_bindings_stratify_aux_equiv e required_level bindings1 bindings2 holey_expr :
-      Proper (eq ==> equivlist ==> eq) holey_expr ->
-      equivlist bindings1 bindings2 ->
-      stratify_aux e required_level bindings1 holey_expr = stratify_aux e required_level bindings2 holey_expr.
-    Proof.
-      assert (trivprop:Proper (eq ==> equivlist ==> eq) (fun (e : nnrc) (_ : list var) => e)) by (repeat red; tauto).
-      revert required_level holey_expr bindings1 bindings2.
-      induction e; intros required_level holey_expr bindings1 bindings2 prope eqb; simpl;
-        do 2 (repeat (first [rewrite eqb
-                            | (erewrite IHe1; try eassumption)
-                            | apply stratify_aux_ext
-                            | apply stratify1_aux_proper
-                            | apply IHe
-                            | apply IHe1
-                            | apply IHe2
-                            | apply IHe3
-                            | apply equivlist_cons
-                            | apply prope]; unfold Proper, respectful; simpl; intros; subst; auto); f_equal).
-    Qed.
-
-    Lemma incl_letvars1 v e1 e2 env :
-      incl (nnrc_vars (NNRCLet v e1 e2)) env ->
-      incl (nnrc_vars e1) env.
-    Proof.
-      intros inclvars.
-      transitivity env; unfold incl, nnrc_vars in *;
-        simpl in *; auto 2; intros.
-      apply inclvars.
-      rewrite in_app_iff in H.
-      repeat rewrite in_app_iff.
-      simpl; rewrite in_app_iff.
-      destruct H; try tauto.
-    Qed.
-    
-    Lemma incl_letvars2 v e1 e2 env :
-      incl (nnrc_vars (NNRCLet v e1 e2)) env ->
-      incl (nnrc_vars e2) (env).
-    Proof.
-      intros inclvars.
-      transitivity env; unfold incl, nnrc_vars in *;
-        simpl in *; auto 2; intros.
-      apply inclvars.
-      rewrite in_app_iff in H.
-      repeat rewrite in_app_iff.
-      simpl; rewrite in_app_iff.
-      destruct H; try tauto.
-      destruct (a == v).
-      - red in e; subst; auto.
-      - left; right.
-        apply remove_in_neq; auto.
-    Qed.
-
-  (*
-    (* our holey contexts preserve contextual equivalence *)
     Definition holey_some_preserver
                h cenv (holey_expr:nnrc->list var -> nnrc) 
-      :=
-        forall e env d,
-          nnrc_core_eval h cenv env e = Some d ->
-        forall holey_bindings holey_bindings' moreenv,
-          incl holey_bindings holey_bindings' ->
-          incl (domain moreenv) holey_bindings' ->
-          nnrc_core_eval h cenv env (holey_expr e holey_bindings) =
-          nnrc_core_eval h cenv (moreenv++env) (holey_expr (NNRCConst d) holey_bindings').
+      := forall v d e env,
+        Forall (data_normalized h) (map snd env) ->
+        incl (nnrc_free_vars e) (domain env) ->
+        ~ In v (domain env) ->
+        nnrc_core_eval h cenv env e = Some d ->
+        nnrc_core_eval h cenv env (holey_expr e (domain env))
+        = nnrc_core_eval h cenv ((v,d)::env) (holey_expr (NNRCVar v) (v::(domain env)))
+    .
 
-    Definition holey_none_preserver h cenv (holey_expr:nnrc->list var -> nnrc)  :=
-      forall e env holey_bindings,
-        nnrc_core_eval h cenv env e = None ->
-        nnrc_core_eval h cenv env (holey_expr e holey_bindings) = None.
+    Definition holey_none_preserver
+               h cenv (holey_expr:nnrc->list var -> nnrc) 
+      := forall e env,
+        Forall (data_normalized h) (map snd env)
+        -> nnrc_core_eval h cenv env e = None
+        -> nnrc_core_eval h cenv env (holey_expr e (domain env)) = None.
+
+(*
+    
+
+    Definition holey_preserver
+               h cenv (holey_expr:nnrc->list var -> nnrc)
+      := forall e env,
+        Forall (data_normalized h) (map snd env) ->        
+        match nnrc_core_eval h cenv env e with
+        | Some d =>
+          forall moreenv e',
+            Forall (data_normalized h) (map snd moreenv) ->
+            nnrc_core_eval h cenv (moreenv++env) e' = Some d ->
+            disjoint (domain moreenv) (domain env) ->
+            nnrc_core_eval h cenv env (holey_expr e (domain env))
+            = nnrc_core_eval h cenv (moreenv++env) (holey_expr e' (domain moreenv++(domain env)))
+        | None => nnrc_core_eval h cenv env (holey_expr e (domain env)) = None
+        end.
+     *)
 
     Lemma stratify1_aux_core_correct
           h cenv (env:bindings)
           (e:nnrc) (required_level:nnrcKind)
-          (holey_bindings:list var) (holey_expr:nnrc->list var->nnrc) :
+          (holey_expr:nnrc->list var->nnrc) :
       Forall (data_normalized h) (map snd cenv) ->
       Forall (data_normalized h) (map snd env) ->
-      holey_none_preserver h cenv holey_expr ->
+      incl (nnrc_free_vars e) (domain env) ->
       holey_some_preserver h cenv holey_expr ->
-      nnrc_core_eval h cenv env (stratify1_aux e required_level holey_bindings holey_expr) =
-      nnrc_core_eval h cenv env (holey_expr e holey_bindings).
+      holey_none_preserver h cenv holey_expr ->
+      nnrc_core_eval h cenv env (stratify1_aux e required_level (domain env) holey_expr) =
+      nnrc_core_eval h cenv env (holey_expr e (domain env)).
     Proof.
-      intros cenv_normalized env_normalized hnp hsp.
+      intros cenv_normalized env_normalized inclfe hsp hnp.
       destruct required_level; simpl; trivial.
-      match_case; simpl.
-      - intros.
-        erewrite (hsp e env d _ _); trivial; try reflexivity.
-        simpl.
-        erewrite (hsp (NNRCVar (fresh_var "stratify" holey_bindings)) _ d).
-        + 
-        + simpl. match_destr; congruence.
-        + unfold incl; simpl; eauto.
-      - intros. rewrite hnp; trivial.
+      symmetry.
+      match_option.
+      - apply hsp; trivial.
+        eapply fresh_var_fresh; eauto.
+      - apply hnp; trivial.
     Qed.
+    
+    Lemma holey_preserver_binop1 h cenv b e1 holey_expr :
+          holey_some_preserver h cenv holey_expr ->
+          holey_some_preserver h cenv
+          (fun (e2n : nnrc) (bound_vars2 : list var) =>
+             holey_expr (NNRCBinop b e1 e2n) bound_vars2).
+    Proof.
+      unfold holey_some_preserver; intros hsp; intros.
+      apply hsp.
+      
+(*      
+
+      generalize (hp e env H); intros hp1.
+      generalize (hp ((NNRCBinop b e1 e)) env H); intros hp2.
+      match_option; intros.
+      - rewrite eqq in *.
+        match_option_in hp2.
+        + apply hp2; trivial.
+          simpl in eqq0.
+          apply some_olift2 in eqq0.
+          destruct eqq0 as [? [??[??]]].
+          simpl.
+          eapply nnrc_core_eval_some_env_extend_disjoint in e0; eauto.
+          rewrite e0.
+          rewrite H1; simpl.
+          rewrite H3 in eqq; invcs eqq.
+          congruence.
+        + rewrite hp2.
+          simpl in eqq0.
+          rewrite eqq in eqq0.
+          unfold olift2 in eqq0.
+          match_option_in eqq0.
+          * admit.
+          * specialize (hp (NNRCBinop b e1 e') (moreenv++env)).
+            simpl in hp.
+
+            eapply (nnrc_core_eval_some_env_extend_disjoint in eqq1; eauto.
+
+            rewrite eqq1 in hp.
           
+          generalize (hp ((NNRCBinop b e1 e')) (moreenv++env)); intros hp3.
+          match_case_in hp3.
+          simpl in hp3.
+          rewrite eqq in eqq0.
+          
+
+          
+
+      - 
+    Qed.
+ *)
+    Admitted.
+    
+    Lemma stratify_aux_core_correct
+          h cenv (env:bindings)
+          (e:nnrc) (required_level:nnrcKind)
+          (holey_expr:nnrc->list var->nnrc) :
+      holey_preserver h cenv holey_expr ->
+      nnrc_eq (stratify_aux e required_level (domain env) holey_expr)
+              (holey_expr e (domain env)).
+              
+      Forall (data_normalized h) (map snd cenv) ->
+      Forall (data_normalized h) (map snd env) ->
+      holey_preserver h cenv holey_expr ->
+      nnrc_core_eval h cenv env (stratify_aux e required_level (domain env) holey_expr) =
+      nnrc_core_eval h cenv env (holey_expr e (domain env)).
+    Proof.
+      revert required_level env holey_expr.
+      nnrc_cases (induction e) Case; intros required_level env holey_expr cenv_normalized env_normalize hp; simpl; trivial.
+      - Case "NNRCBinop"%string.
+        admit.
+        (*
+        rewrite IHe1; trivial.
+        + rewrite IHe2; trivial.
+          * red; intros.
+            { specialize (hp e env).
+              match_option; intros.
+              - 
+admit. (*            
+            apply (hsp moreenv).
+            apply hsp; trivial.
+            simpl.
+            rewrite H0; trivial.
+          * 
+        + red; intros.
+          repeat rewrite IHe2; trivial.
+          * apply hp; simpl; trivial.
+            rewrite H0; trivial.
+          * red; intros.
+            apply hp; trivial.
+            simpl; rewrite H2; trivial.
+          * red; intros.
+            apply hp; trivial.
+            simpl; rewrite H2; trivial. *)
+*)
+      - Case "NNRCUnop"%string.
+        admit.
+      - Case "NNRCLet"%string.
+        rewrite IHe1; trivial.
+        + rewrite stratify1_aux_core_correct; trivial.
+           generalize (hp (NNRCLet v e1
+                                   (stratify_aux e2 nnrcStmt (v :: domain env) (fun (e : nnrc) (_ : list var) => e))) env env_normalize); intros hp1.
+           generalize (hp (NNRCLet v e1 e2) env env_normalize); intros hp2.
+           match_option_in hp2; match_option_in hp1.
+          * admit.
+          * rewrite hp1.
+            admit.
+          * rewrite hp2.
+            admit.
+          * rewrite hp1, hp2; trivial.
+        + red; unfold stratify1_aux; intros.
+          destruct required_level; simpl.
+          match_option; intros.
+          * rewrite H1.
+            {  rewrite IHe2; trivial.
+              - specialize (IHe2 nnrcStmt (((v, d) :: moreenv ++ env0))).
+                simpl in IHe2.
+                repeat rewrite domain_app in IHe2.
+                rewrite IHe2; trivial.
+                replace (((v, d) :: moreenv ++ env)) with (((v, d) :: nil ++ moreenv ++ env)) by (simpl; trivial).
+                rewrite <- nnrc_core_eval_some_env_extend_disjoint.
+                + 
+              repeat match_option.
+              - 
+            
+          * simpl.
+    Qed.
+
     Lemma stratify_aux_core_correct
           h cenv (env:bindings)
           (e:nnrc) (required_level:nnrcKind)
