coq/Utils/CoqLibAdd.v
@@ -951,7 +951,7 @@ Ltac match_option
   := let eqq := fresh "eqq" in
      match goal with
        [|- context [match ?x with | Some _ => _ | None => _ end]] =>
-       case_eq x end; [ intros ? eqq | intros eqq]; rewrite eqq;
+       case_eq x end; [ intros ? eqq | intros eqq]; try rewrite eqq;
      trivial; try discriminate.
 
 Ltac match_option_in H
